revert :(

src/Init/Data/Range/Polymorphic/RangeIterator.lean
@@ -88,16 +88,17 @@ theorem Iterator.step_eq_monadicStep [UpwardEnumerable α] [LE α] [DecidableLE 
 @[always_inline, inline]
 instance [UpwardEnumerable α] [LE α] [DecidableLE α] :
     Iterator (Rxc.Iterator α) Id α where
-  step it := return Iterator.Monadic.step it
+  IsPlausibleStep it step := step = Iterator.Monadic.step it
+  step it := pure <| .deflate <| ⟨Iterator.Monadic.step it, rfl⟩
 
 theorem Iterator.Monadic.isPlausibleStep_iff [UpwardEnumerable α] [LE α] [DecidableLE α]
     {it : IterM (α := Rxc.Iterator α) Id α} {step} :
     it.IsPlausibleStep step ↔ step = Iterator.Monadic.step it := by
-  simp [IterM.IsPlausibleStep, MonadAttach.CanReturn, Iterators.Iterator.step, eq_comm]
+  exact Iff.rfl
 
 theorem Iterator.Monadic.step_eq_step [UpwardEnumerable α] [LE α] [DecidableLE α]
     {it : IterM (α := Rxc.Iterator α) Id α} :
-    it.step = pure (Iterator.Monadic.step it) := by
+    it.step = pure (.deflate ⟨Iterator.Monadic.step it, isPlausibleStep_iff.mpr rfl⟩) := by
   simp [IterM.step, Iterators.Iterator.step]
 
 theorem Iterator.isPlausibleStep_iff [UpwardEnumerable α] [LE α] [DecidableLE α]
@@ -115,7 +116,7 @@ theorem Iterator.isPlausibleStep_iff [UpwardEnumerable α] [LE α] [DecidableLE 
 
 theorem Iterator.step_eq_step [UpwardEnumerable α] [LE α] [DecidableLE α]
     {it : Iter (α := Rxc.Iterator α) α} :
-    it.step = Iterator.step it := by
+    it.step = ⟨Iterator.step it, isPlausibleStep_iff.mpr rfl⟩ := by
   simp [Iter.step, step_eq_monadicStep, Monadic.step_eq_step, IterM.Step.toPure]
 
 instance Iterator.instIteratorCollect [UpwardEnumerable α] [LE α] [DecidableLE α]
@@ -135,7 +136,7 @@ theorem Iterator.Monadic.isPlausibleOutput_iff
     it.IsPlausibleOutput a ↔
       it.internalState.next = some a ∧
         a ≤ it.internalState.upperBound := by
-  simp only [IterM.IsPlausibleOutput, isPlausibleStep_iff, step]
+  simp [IterM.IsPlausibleOutput, isPlausibleStep_iff, Monadic.step]
   split
   · simp [*]
   · constructor
@@ -173,7 +174,7 @@ theorem Iterator.Monadic.isPlausibleSuccessorOf_iff
   constructor
   · rintro ⟨step, h, h'⟩
     cases h'
-    simp only [Iterators.Iterator.step, Monadic.step, Id.run_pure] at h
+    simp only [Monadic.step] at h
     split at h
     · cases h
     · split at h
@@ -183,7 +184,8 @@ theorem Iterator.Monadic.isPlausibleSuccessorOf_iff
       · cases h
   · rintro ⟨a, h, hP, h'⟩
     refine ⟨.yield it' a, rfl, ?_⟩
-    simp only [IterM.IsPlausibleStep, MonadAttach.CanReturn, Iterators.Iterator.step, step, h, hP]
+    simp only [IterM.IsPlausibleStep, Iterator.IsPlausibleStep, step, h, hP, ↓reduceIte,
+      IterStep.yield.injEq, and_true]
     simp [h'.1, ← h'.2]
 
 theorem Iterator.isPlausibleSuccessorOf_iff
@@ -243,11 +245,10 @@ private def Iterator.instFinitenessRelation [UpwardEnumerable α] [LE α] [Decid
       intro bound
       constructor
       intro it' ⟨step, hs₁, hs₂⟩
-      simp only [IterM.IsPlausibleStep, MonadAttach.CanReturn, Iterators.Iterator.step,
-        Monadic.step, Id.run_pure] at hs₂
-      simp [← hs₂, IterStep.successor] at hs₁
-    simp only [IterM.IsPlausibleSuccessorOf, IterM.IsPlausibleStep, MonadAttach.CanReturn,
-      Iterators.Iterator.step, Monadic.step] at hnone ⊢
+      simp only [IterM.IsPlausibleStep, Iterator.IsPlausibleStep, Monadic.step] at hs₂
+      simp [hs₂, IterStep.successor] at hs₁
+    simp only [IterM.IsPlausibleSuccessorOf, IterM.IsPlausibleStep, Iterator.IsPlausibleStep,
+      Monadic.step, exists_eq_right] at hnone ⊢
     match it with
     | ⟨⟨none, _⟩⟩ => apply hnone
     | ⟨⟨some init, bound⟩⟩ =>
@@ -266,21 +267,17 @@ private def Iterator.instFinitenessRelation [UpwardEnumerable α] [LE α] [Decid
           simp only [hs]
           intro h
           split at h
-          · obtain ⟨_, h, rfl⟩ := h
-            cases h
+          · cases h
             apply hnone
-          · obtain ⟨_, h, rfl⟩ := h
-            cases h
+          · cases h
         | some a =>
           intro h
           simp only [hs] at h hn
           specialize ih _ hn
           split at h
-          · obtain ⟨_, h, rfl⟩ := h
-            cases h
+          · cases h
             exact ih
-          · obtain ⟨_, h, rfl⟩ := h
-            cases h
+          · cases h
   subrelation := id
 
 @[no_expose]
@@ -297,7 +294,7 @@ private def Iterator.instProductivenessRelation [UpwardEnumerable α] [LE α] [D
   subrelation {it it'} h := by
     exfalso
     simp only [IterM.IsPlausibleSkipSuccessorOf, IterM.IsPlausibleStep,
-      MonadAttach.CanReturn, Iterators.Iterator.step, Monadic.step, Id.run_pure] at h
+      Iterator.IsPlausibleStep, Monadic.step] at h
     split at h
     · cases h
     · split at h
@@ -313,19 +310,12 @@ instance Iterator.instProductive [UpwardEnumerable α] [LE α] [DecidableLE α]
 instance Iterator.instIteratorAccess [UpwardEnumerable α] [LE α] [DecidableLE α]
     [LawfulUpwardEnumerable α] [LawfulUpwardEnumerableLE α] :
     IteratorAccess (Rxc.Iterator α) Id where
-  nextAtIdx? it n := match it.internalState.next.bind (UpwardEnumerable.succMany? n) with
+  nextAtIdx? it n := ⟨match it.internalState.next.bind (UpwardEnumerable.succMany? n) with
     | none => .done
     | some next => if next ≤ it.internalState.upperBound then
         .yield ⟨⟨UpwardEnumerable.succ? next, it.internalState.upperBound⟩⟩ next
       else
-        .done
-
-instance Iterator.instLawfulIteratorAccess [UpwardEnumerable α] [LE α] [DecidableLE α]
-    [LawfulUpwardEnumerable α] [LawfulUpwardEnumerableLE α] :
-    LawfulIteratorAccess (Rxc.Iterator α) Id where
-  isPlausibleNthOutputStep_of_canReturn {it n s} h := by
-      simp only [MonadAttach.CanReturn, IteratorAccess.nextAtIdx?] at h
-      cases h
+        .done, (by
       induction n generalizing it
       · split <;> rename_i heq
         · apply IterM.IsPlausibleNthOutputStep.done
@@ -353,7 +343,7 @@ instance Iterator.instLawfulIteratorAccess [UpwardEnumerable α] [LE α] [Decida
             simp only [Monadic.isPlausibleStep_iff, Monadic.step, heq']
           · rename_i out
             simp only [heq', Option.bind_some, succMany?_add_one_eq_succ?_bind_succMany?] at heq
-            specialize ih (it := ⟨⟨UpwardEnumerable.succ? out, it.internalState.upperBound⟩⟩)
+            specialize ih ⟨⟨UpwardEnumerable.succ? out, it.internalState.upperBound⟩⟩
             simp only [heq] at ih
             by_cases heq'' : out ≤ it.internalState.upperBound
             · apply IterM.IsPlausibleNthOutputStep.yield
@@ -369,7 +359,7 @@ instance Iterator.instLawfulIteratorAccess [UpwardEnumerable α] [LE α] [Decida
           simp only [heq', Option.bind_some] at heq
           have hle : UpwardEnumerable.LE out _ := ⟨n + 1, heq⟩
           simp only [succMany?_add_one_eq_succ?_bind_succMany?] at heq
-          specialize ih (it := ⟨⟨UpwardEnumerable.succ? out, it.internalState.upperBound⟩⟩)
+          specialize ih ⟨⟨UpwardEnumerable.succ? out, it.internalState.upperBound⟩⟩
           simp only [heq] at ih
           by_cases hout : out ≤ it.internalState.upperBound
           · apply IterM.IsPlausibleNthOutputStep.yield
@@ -385,12 +375,11 @@ instance Iterator.instLawfulIteratorAccess [UpwardEnumerable α] [LE α] [Decida
             simp only [this, ↓reduceIte]
             simp only [this, ↓reduceIte] at ih
             apply IterM.IsPlausibleNthOutputStep.done
-            simp [Monadic.isPlausibleStep_iff, Monadic.step, heq', hout]
+            simp [Monadic.isPlausibleStep_iff, Monadic.step, heq', hout])⟩
 
 instance Iterator.instLawfulDeterministicIterator [UpwardEnumerable α] [LE α] [DecidableLE α] :
     LawfulDeterministicIterator (Rxc.Iterator α) Id where
-  isPlausibleStep_eq_eq it := ⟨Monadic.step it, by
-      simp [IterM.IsPlausibleStep, MonadAttach.CanReturn, Iterators.Iterator.step, eq_comm]⟩
+  isPlausibleStep_eq_eq it := ⟨Monadic.step it, rfl⟩
 
 theorem Iterator.Monadic.isPlausibleIndirectOutput_iff
     [UpwardEnumerable α] [LE α] [DecidableLE α] [LawfulUpwardEnumerableLE α]
@@ -455,23 +444,23 @@ loop implementation.
 @[always_inline, inline]
 instance Iterator.instIteratorLoop [UpwardEnumerable α] [LE α] [DecidableLE α]
     [LawfulUpwardEnumerable α] [LawfulUpwardEnumerableLE α]
-    {n : Type u → Type w} [Monad n] [MonadAttach n] :
+    {n : Type u → Type w} [Monad n] :
     IteratorLoop (Rxc.Iterator α) Id n where
-  forIn _ γ it init f :=
+  forIn _ γ Pl it init f :=
     match it with
     | ⟨⟨some next, upperBound⟩⟩ =>
-      loop γ (next ≤ ·) (fun a b hab hna => ?hle) upperBound init next ?hle'' (fun a ha c => f a ?hf c)
+      loop γ Pl (next ≤ ·) (fun a b hab hna => ?hle) upperBound init next ?hle'' (fun a ha₁ ha₂ c => f a ?hf c)
     | ⟨⟨none, _⟩⟩ => return init
   where
     @[always_inline, inline]
-    loop γ (LargeEnough : α → Prop) (hl : ∀ a b : α, a ≤ b → LargeEnough a → LargeEnough b)
+    loop γ (Pl : α → γ → ForInStep γ → Prop) (LargeEnough : α → Prop) (hl : ∀ a b : α, a ≤ b → LargeEnough a → LargeEnough b)
         (upperBound : α) (acc : γ) (next : α) (h : LargeEnough next)
-        (f : (out : α) → LargeEnough out ∧ out ≤ upperBound → (c : γ) → n (ForInStep γ)) : n γ :=
+        (f : (out : α) → LargeEnough out → out ≤ upperBound → (c : γ) → n (Subtype (Pl out c))) : n γ :=
       haveI : Nonempty γ := ⟨acc⟩
-      WellFounded.extrinsicFix₃ (C₃ := fun _ _ _ => n γ) (InvImage (IteratorLoop.rel _ Id (fun out h c => MonadAttach.CanReturn <| f out h c)) (fun x => (⟨Rxc.Iterator.mk (some x.1) upperBound⟩, x.2.1)))
+      WellFounded.extrinsicFix₃ (C₃ := fun _ _ _ => n γ) (InvImage (IteratorLoop.rel _ Id Pl) (fun x => (⟨Rxc.Iterator.mk (some x.1) upperBound⟩, x.2.1)))
         (fun next acc (h : LargeEnough next) G => do
           if hu : next ≤ upperBound then
-            match ← MonadAttach.attach (f next ⟨h, hu⟩ acc) with
+            match ← f next h hu acc with
             | ⟨.yield acc', h'⟩ =>
               match hs : UpwardEnumerable.succ? next with
               | some next' => G next' acc' (hl _ _ ?hle' h) ?decreasing
@@ -482,9 +471,9 @@ instance Iterator.instIteratorLoop [UpwardEnumerable α] [LE α] [DecidableLE α
   finally
     case hf =>
       rw [Monadic.isPlausibleIndirectOutput_iff]
-      simp only [UpwardEnumerable.le_iff] at ha
-      obtain ⟨n, hn⟩ := ha.1
-      exact ⟨n, hn, by simpa [UpwardEnumerable.le_iff] using ha.2⟩
+      simp only [UpwardEnumerable.le_iff] at ha₁
+      obtain ⟨n, hn⟩ := ha₁
+      exact ⟨n, hn, ha₂⟩
     case hle =>
       simp only [UpwardEnumerable.le_iff] at hna hab ⊢
       exact UpwardEnumerable.le_trans hna hab
@@ -500,18 +489,19 @@ instance Iterator.instIteratorLoop [UpwardEnumerable α] [LE α] [DecidableLE α
 
 private noncomputable def Iterator.instIteratorLoop.loop.wf [UpwardEnumerable α] [LE α] [DecidableLE α]
     [LawfulUpwardEnumerable α] [LawfulUpwardEnumerableLE α]
-    {n : Type u → Type w} [Monad n] [MonadAttach n] (γ : Type u)
+    {n : Type u → Type w} [Monad n] (γ : Type u)
+    (Pl : α → γ → ForInStep γ → Prop)
+    (wf : IteratorLoop.WellFounded (Rxc.Iterator α) Id Pl)
     (LargeEnough : α → Prop) (hl : ∀ a b : α, a ≤ b → LargeEnough a → LargeEnough b)
     (upperBound : α) (acc : γ) (next : α) (h : LargeEnough next)
-    (f : (out : α) → LargeEnough out ∧ out ≤ upperBound → (c : γ) → n (ForInStep γ))
-    (wf : IteratorLoop.WellFounded (Rxc.Iterator α) Id (fun out h c => MonadAttach.CanReturn <| f out h c)) :
+    (f : (out : α) → LargeEnough out → out ≤ upperBound → (c : γ) → n (Subtype (fun s : ForInStep γ => Pl out c s))) :
     n γ := do
   if hu : next ≤ upperBound then
-    match ← MonadAttach.attach (f next ⟨h, hu⟩ acc) with
+    match ← f next h hu acc with
     | ⟨.yield acc', _⟩ =>
       match hs : UpwardEnumerable.succ? next with
       | some next' =>
-        loop.wf γ LargeEnough hl upperBound acc' next' (hl _ _ ?hle h) f wf
+        loop.wf γ Pl wf LargeEnough hl upperBound acc' next' (hl _ _ ?hle h) f
       | none => return acc'
     | ⟨.done acc', _⟩ => return acc'
   else
@@ -526,14 +516,14 @@ where finally
     simpa [succMany?_one] using hs
 
 private theorem Iterator.instIteratorLoop.loop_eq_wf [UpwardEnumerable α] [LE α] [DecidableLE α]
-    [LawfulUpwardEnumerable α] [LawfulUpwardEnumerableLE α] [Monad n] [MonadAttach n] [LawfulMonad n]
-    {γ LargeEnough hl upperBound} {next hn} {acc} (f wf) :
-    loop γ LargeEnough hl upperBound acc next hn f =
-      loop.wf (α := α) (n := n) γ LargeEnough hl upperBound acc next hn f wf := by
+    [LawfulUpwardEnumerable α] [LawfulUpwardEnumerableLE α] [Monad n] [LawfulMonad n]
+    {γ LargeEnough hl upperBound} {next hn} {acc} (Pl wf f) :
+    loop γ Pl LargeEnough hl upperBound acc next hn f =
+      loop.wf (α := α) (n := n) γ Pl wf LargeEnough hl upperBound acc next hn f := by
   haveI : Nonempty γ := ⟨acc⟩
   rw [loop, WellFounded.extrinsicFix₃_eq_fix]; rotate_left
   · exact InvImage.wf _ wf
-  · fun_induction loop.wf γ LargeEnough hl upperBound acc  next hn f wf
+  · fun_induction loop.wf γ Pl wf LargeEnough hl upperBound acc  next hn f
     · rw [WellFounded.fix_eq]
       simp only [↓reduceDIte, *]
       apply bind_congr; intro forInStep
@@ -548,91 +538,76 @@ private theorem Iterator.instIteratorLoop.loop_eq_wf [UpwardEnumerable α] [LE �
 
 private theorem Iterator.instIteratorLoop.loopWf_eq [UpwardEnumerable α] [LE α] [DecidableLE α]
     [LawfulUpwardEnumerable α] [LawfulUpwardEnumerableLE α]
-    {n : Type u → Type w} [Monad n] [MonadAttach n] [LawfulMonad n] [LawfulMonadAttach n]
-    (γ : Type u) {lift}
-    [instLawfulMonadLiftFunction : Std.Internal.LawfulMonadLiftBindFunction (m := Id) (n := n) lift]
+    {n : Type u → Type w} [Monad n] [LawfulMonad n] (γ : Type u)
+    {lift} [instLawfulMonadLiftFunction : Std.Internal.LawfulMonadLiftBindFunction (m := Id) (n := n) lift]
+    (Pl : α → γ → ForInStep γ → Prop)
+    (wf : IteratorLoop.WellFounded (Rxc.Iterator α) Id Pl)
     (LargeEnough : α → Prop) (hl : ∀ a b : α, a ≤ b → LargeEnough a → LargeEnough b)
     (upperBound : α) (acc : γ) (next : α) (h : LargeEnough next)
-    (f : (out : α) → LargeEnough out ∧ out ≤ upperBound → (c : γ) → n (ForInStep γ))
-    (wf : IteratorLoop.WellFounded (Rxc.Iterator α) Id _) :
-    loop.wf γ LargeEnough hl upperBound acc next h f wf = (do
+    (f : (out : α) → LargeEnough out → out ≤ upperBound → (c : γ) → n (Subtype (fun s : ForInStep γ => Pl out c s))) :
+    loop.wf γ Pl wf LargeEnough hl upperBound acc next h f = (do
       if hu : next ≤ upperBound then
-        match ← MonadAttach.attach (f next ⟨h, hu⟩ acc) with
+        match ← f next h hu acc with
         | ⟨.yield acc', _⟩ =>
           letI it' : IterM (α := Rxc.Iterator α) Id α := ⟨⟨succ? next, upperBound⟩⟩
-          IterM.DefaultConsumers.forIn' (m := Id) (n := n) lift γ it' acc'
-            (fun a => LargeEnough a ∧ a ≤ upperBound) (fun a h => by
-              rw [Monadic.isPlausibleIndirectOutput_iff] at h
-              obtain ⟨n, h₁, h₂⟩ := h
-              apply And.intro
-              · apply hl next a _ h
-                rw [UpwardEnumerable.le_iff]
-                simp only [it', ← UpwardEnumerable.succMany?_add_one_eq_succ?_bind_succMany?] at h₁
-                exact ⟨n + 1, h₁⟩
-              · exact h₂)
-            fun next' h acc' => f next' h acc'
+          IterM.DefaultConsumers.forIn' (m := Id) (n := n) lift γ Pl it' acc'
+            it'.IsPlausibleIndirectOutput (fun _ => id)
+            fun next' h acc' => f next'
+              (by
+                refine hl next next' ?_ ‹_›
+                simp only [it', Monadic.isPlausibleIndirectOutput_iff,
+                  ← succMany?_add_one_eq_succ?_bind_succMany?] at h
+                exact UpwardEnumerable.le_iff.mpr ⟨h.choose + 1, h.choose_spec.1⟩)
+              (by
+                simp only [it', Monadic.isPlausibleIndirectOutput_iff] at h
+                exact h.choose_spec.2)
+              acc'
         | ⟨.done acc', _⟩ => return acc'
       else return acc) := by
-  fun_induction loop.wf γ LargeEnough hl upperBound acc next h f wf
-  · rename_i ih
-    simp only [↓reduceDIte, *]
-    apply bind_congr; intro forInStep
-    split
-    · split
-      · rw [ih _ ‹_› _ ‹_›]
-        rw [IterM.DefaultConsumers.forIn'_eq_match_step (lift := lift) (wf := wf)]; rotate_left
-        · simp only [Monadic.step_eq_step, MonadAttach.CanReturn, MonadAttach.attach, Monadic.step,
-            instLawfulMonadLiftFunction.liftBind_pure, *]
+  haveI : Nonempty γ := ⟨acc⟩
+  rw [loop.wf]
+  congr 1; ext hu
+  apply bind_congr; intro forInStep
+  split
+  · split
+    · rw [loopWf_eq (lift := lift) _ Pl wf]
+      rw [IterM.DefaultConsumers.forIn'_eq_match_step (lift := lift) Pl wf]; rotate_left
+      · simp only [Monadic.step_eq_step, Monadic.step,
+          Shrink.inflate_deflate, instLawfulMonadLiftFunction.liftBind_pure, *]
+        split
+        · apply bind_congr; intro forInStep
           split
-          · conv => rhs; simp only [Id.run_pure, ← LawfulMonadAttach.map_attach (x := f _ _ _),
-              bind_map_left]
-            apply bind_congr; intro forInStep
-            split
-            · apply IterM.DefaultConsumers.forIn'_eq_forIn' (wf := wf) (wf' := wf)
-              intros; simp
-            · simp
+          · apply IterM.DefaultConsumers.forIn'_eq_forIn' Pl wf <;> (intros; rfl)
           · simp
-      · rw [IterM.DefaultConsumers.forIn'_eq_match_step wf]
-        simp [MonadAttach.CanReturn, MonadAttach.attach, Monadic.step_eq_step, Monadic.step,
-          instLawfulMonadLiftFunction.liftBind_pure, *]
-    · simp
-  · simp only [right_eq_dite_iff]
-    intro h
-    exact Not.elim ‹_› h
-
-theorem _root_.Std.Iterators.IteratorLoop.wellFounded_congr [MonadAttach m] [Iterator α m β] {P Q : β → Prop}
-    {Pl : (out : β) → P out → γ → ForInStep γ → Prop}
-    (h : P = Q) :
-    IteratorLoop.WellFounded α m Pl ↔ IteratorLoop.WellFounded α m (fun b hb => Pl b (h ▸ hb)) := by
-  cases h; rfl
+        · simp
+    · rw [IterM.DefaultConsumers.forIn'_eq_match_step Pl wf]
+      simp [Monadic.step_eq_step, Monadic.step, instLawfulMonadLiftFunction.liftBind_pure, *]
+  · simp
+termination_by IteratorLoop.WithWF.mk ⟨⟨some next, upperBound⟩⟩ acc (hwf := wf)
+decreasing_by
+  simp [IteratorLoop.rel, Monadic.isPlausibleStep_iff, Monadic.step, *]
 
 instance Iterator.instLawfulIteratorLoop [UpwardEnumerable α] [LE α] [DecidableLE α]
     [LawfulUpwardEnumerable α] [LawfulUpwardEnumerableLE α]
-    {n : Type u → Type w} [Monad n] [MonadAttach n] [LawfulMonadAttach n] [LawfulMonad n] :
+    {n : Type u → Type w} [Monad n] [LawfulMonad n] :
     LawfulIteratorLoop (Rxc.Iterator α) Id n where
   lawful := by
-    intro lift instLawfulMonadLiftFunction γ it init f wf
+    intro lift instLawfulMonadLiftFunction γ it init Pl wf f
     simp only [IteratorLoop.defaultImplementation, IteratorLoop.forIn,
-      IterM.DefaultConsumers.forIn'_eq_wf f wf]
+      IterM.DefaultConsumers.forIn'_eq_wf Pl wf]
     rw [IterM.DefaultConsumers.forIn'.wf]
     split; rotate_left
-    · simp [Monadic.step_eq_step, MonadAttach.CanReturn, MonadAttach.attach, Monadic.step,
-        Internal.LawfulMonadLiftBindFunction.liftBind_pure]
-    rename_i lo next f
-    have wf' := wf
-    rw [IteratorLoop.wellFounded_congr (Q := fun b => lo ≤ b ∧ b ≤ next)] at wf'; rotate_left
-    · ext
-      simp [Monadic.isPlausibleIndirectOutput_iff, ← UpwardEnumerable.le_iff_exists, ← UpwardEnumerable.le_iff]
-    rw [instIteratorLoop.loop_eq_wf (wf := wf'), instIteratorLoop.loopWf_eq (lift := lift)]; rotate_left
-    simp only [Monadic.step_eq_step, MonadAttach.CanReturn, MonadAttach.attach, Monadic.step,
-      instLawfulMonadLiftFunction.liftBind_pure]
+    · simp [Monadic.step_eq_step, Monadic.step, Internal.LawfulMonadLiftBindFunction.liftBind_pure]
+    rename_i next _
+    rw [instIteratorLoop.loop_eq_wf Pl wf, instIteratorLoop.loopWf_eq (lift := lift)]
+    simp only [Monadic.step_eq_step, Monadic.step, instLawfulMonadLiftFunction.liftBind_pure,
+      Shrink.inflate_deflate]
     split
     · apply bind_congr; intro forInStep
       split
       · simp only
-        rw [← IterM.DefaultConsumers.forIn'_eq_wf _ wf]
-        apply IterM.DefaultConsumers.forIn'_eq_forIn' wf' wf
-        intros; rfl
+        rw [← IterM.DefaultConsumers.forIn'_eq_wf Pl wf _]
+        apply IterM.DefaultConsumers.forIn'_eq_forIn' Pl wf <;> all_goals (intros; rfl)
       · simp
     · simp
 
@@ -693,16 +668,17 @@ theorem Iterator.step_eq_monadicStep [UpwardEnumerable α] [LT α] [DecidableLT 
 @[always_inline, inline]
 instance [UpwardEnumerable α] [LT α] [DecidableLT α] :
     Iterator (Rxo.Iterator α) Id α where
-  step it := return Iterator.Monadic.step it
+  IsPlausibleStep it step := step = Iterator.Monadic.step it
+  step it := pure (.deflate ⟨Iterator.Monadic.step it, rfl⟩)
 
 theorem Iterator.Monadic.isPlausibleStep_iff [UpwardEnumerable α] [LT α] [DecidableLT α]
     {it : IterM (α := Rxo.Iterator α) Id α} {step} :
     it.IsPlausibleStep step ↔ step = Iterator.Monadic.step it := by
-  simp [IterM.IsPlausibleStep, MonadAttach.CanReturn, Iterators.Iterator.step, eq_comm]
+  exact Iff.rfl
 
 theorem Iterator.Monadic.step_eq_step [UpwardEnumerable α] [LT α] [DecidableLT α]
     {it : IterM (α := Rxo.Iterator α) Id α} :
-    it.step = pure (Iterator.Monadic.step it) := by
+    it.step = pure (.deflate ⟨Iterator.Monadic.step it, isPlausibleStep_iff.mpr rfl⟩) := by
   simp [IterM.step, Iterators.Iterator.step]
 
 theorem Iterator.isPlausibleStep_iff [UpwardEnumerable α] [LT α] [DecidableLT α]
@@ -720,7 +696,7 @@ theorem Iterator.isPlausibleStep_iff [UpwardEnumerable α] [LT α] [DecidableLT 
 
 theorem Iterator.step_eq_step [UpwardEnumerable α] [LT α] [DecidableLT α]
     {it : Iter (α := Rxo.Iterator α) α} :
-    it.step = Iterator.step it := by
+    it.step = ⟨Iterator.step it, isPlausibleStep_iff.mpr rfl⟩ := by
   simp [Iter.step, step_eq_monadicStep, Monadic.step_eq_step, IterM.Step.toPure]
 
 instance Iterator.instIteratorCollect [UpwardEnumerable α] [LT α] [DecidableLT α]
@@ -778,7 +754,7 @@ theorem Iterator.Monadic.isPlausibleSuccessorOf_iff
   constructor
   · rintro ⟨step, h, h'⟩
     cases h'
-    simp only [Iterators.Iterator.step, Monadic.step, Id.run_pure] at h
+    simp only [Monadic.step] at h
     split at h
     · cases h
     · split at h
@@ -788,7 +764,8 @@ theorem Iterator.Monadic.isPlausibleSuccessorOf_iff
       · cases h
   · rintro ⟨a, h, hP, h'⟩
     refine ⟨.yield it' a, rfl, ?_⟩
-    simp only [IterM.IsPlausibleStep, MonadAttach.CanReturn, Iterators.Iterator.step, step, h, hP]
+    simp only [IterM.IsPlausibleStep, Iterator.IsPlausibleStep, step, h, hP, ↓reduceIte,
+      IterStep.yield.injEq, and_true]
     simp [h'.1, ← h'.2]
 
 theorem Iterator.isPlausibleSuccessorOf_iff
@@ -848,11 +825,10 @@ private def Iterator.instFinitenessRelation [UpwardEnumerable α] [LT α] [Decid
       intro bound
       constructor
       intro it' ⟨step, hs₁, hs₂⟩
-      simp only [IterM.IsPlausibleStep, MonadAttach.CanReturn, Iterators.Iterator.step,
-        Monadic.step, Id.run_pure] at hs₂
-      simp [← hs₂, IterStep.successor] at hs₁
-    simp only [IterM.IsPlausibleSuccessorOf, IterM.IsPlausibleStep, MonadAttach.CanReturn,
-      Iterators.Iterator.step, Monadic.step] at hnone ⊢
+      simp only [IterM.IsPlausibleStep, Iterator.IsPlausibleStep, Monadic.step] at hs₂
+      simp [hs₂, IterStep.successor] at hs₁
+    simp only [IterM.IsPlausibleSuccessorOf, IterM.IsPlausibleStep, Iterator.IsPlausibleStep,
+      Monadic.step, exists_eq_right] at hnone ⊢
     match it with
     | ⟨⟨none, _⟩⟩ => apply hnone
     | ⟨⟨some init, bound⟩⟩ =>
@@ -871,21 +847,17 @@ private def Iterator.instFinitenessRelation [UpwardEnumerable α] [LT α] [Decid
           simp only [hs]
           intro h
           split at h
-          · obtain ⟨_, h, rfl⟩ := h
-            cases h
+          · cases h
             apply hnone
-          · obtain ⟨_, h, rfl⟩ := h
-            cases h
+          · cases h
         | some a =>
           intro h
           simp only [hs] at h hn
           specialize ih _ hn
           split at h
-          · obtain ⟨_, h, rfl⟩ := h
-            cases h
+          · cases h
             exact ih
-          · obtain ⟨_, h, rfl⟩ := h
-            cases h
+          · cases h
   subrelation := id
 
 @[no_expose]
@@ -902,7 +874,7 @@ private def Iterator.instProductivenessRelation [UpwardEnumerable α] [LT α] [D
   subrelation {it it'} h := by
     exfalso
     simp only [IterM.IsPlausibleSkipSuccessorOf, IterM.IsPlausibleStep,
-      MonadAttach.CanReturn, Iterators.Iterator.step, Monadic.step, Id.run_pure] at h
+      Iterator.IsPlausibleStep, Monadic.step] at h
     split at h
     · cases h
     · split at h
@@ -918,19 +890,12 @@ instance Iterator.instProductive [UpwardEnumerable α] [LT α] [DecidableLT α]
 instance Iterator.instIteratorAccess [UpwardEnumerable α] [LT α] [DecidableLT α]
     [LawfulUpwardEnumerable α] [LawfulUpwardEnumerableLT α] :
     IteratorAccess (Rxo.Iterator α) Id where
-  nextAtIdx? it n := match it.internalState.next.bind (UpwardEnumerable.succMany? n) with
+  nextAtIdx? it n := ⟨match it.internalState.next.bind (UpwardEnumerable.succMany? n) with
     | none => .done
     | some next => if next < it.internalState.upperBound then
         .yield ⟨⟨UpwardEnumerable.succ? next, it.internalState.upperBound⟩⟩ next
       else
-        .done
-
-instance Iterator.instLawfulIteratorAccess [UpwardEnumerable α] [LT α] [DecidableLT α]
-    [LawfulUpwardEnumerable α] [LawfulUpwardEnumerableLT α] :
-    LawfulIteratorAccess (Rxo.Iterator α) Id where
-  isPlausibleNthOutputStep_of_canReturn {it n s} h := by
-      simp only [MonadAttach.CanReturn, IteratorAccess.nextAtIdx?] at h
-      cases h
+        .done, (by
       induction n generalizing it
       · split <;> rename_i heq
         · apply IterM.IsPlausibleNthOutputStep.done
@@ -958,7 +923,7 @@ instance Iterator.instLawfulIteratorAccess [UpwardEnumerable α] [LT α] [Decida
             simp only [Monadic.isPlausibleStep_iff, Monadic.step, heq']
           · rename_i out
             simp only [heq', Option.bind_some, succMany?_add_one_eq_succ?_bind_succMany?] at heq
-            specialize ih (it := ⟨⟨UpwardEnumerable.succ? out, it.internalState.upperBound⟩⟩)
+            specialize ih ⟨⟨UpwardEnumerable.succ? out, it.internalState.upperBound⟩⟩
             simp only [heq] at ih
             by_cases heq'' : out < it.internalState.upperBound
             · apply IterM.IsPlausibleNthOutputStep.yield
@@ -974,7 +939,7 @@ instance Iterator.instLawfulIteratorAccess [UpwardEnumerable α] [LT α] [Decida
           simp only [heq', Option.bind_some] at heq
           have hlt : UpwardEnumerable.LT out _ := ⟨n, heq⟩
           simp only [succMany?_add_one_eq_succ?_bind_succMany?] at heq
-          specialize ih (it := ⟨⟨UpwardEnumerable.succ? out, it.internalState.upperBound⟩⟩)
+          specialize ih ⟨⟨UpwardEnumerable.succ? out, it.internalState.upperBound⟩⟩
           simp only [heq] at ih
           by_cases hout : out < it.internalState.upperBound
           · apply IterM.IsPlausibleNthOutputStep.yield
@@ -990,12 +955,11 @@ instance Iterator.instLawfulIteratorAccess [UpwardEnumerable α] [LT α] [Decida
             simp only [this, ↓reduceIte]
             simp only [this, ↓reduceIte] at ih
             apply IterM.IsPlausibleNthOutputStep.done
-            simp [Monadic.isPlausibleStep_iff, Monadic.step, heq', hout]
+            simp [Monadic.isPlausibleStep_iff, Monadic.step, heq', hout])⟩
 
 instance Iterator.instLawfulDeterministicIterator [UpwardEnumerable α] [LT α] [DecidableLT α] :
     LawfulDeterministicIterator (Rxo.Iterator α) Id where
-  isPlausibleStep_eq_eq it := ⟨Monadic.step it, by
-      simp [IterM.IsPlausibleStep, MonadAttach.CanReturn, Iterators.Iterator.step, eq_comm]⟩
+  isPlausibleStep_eq_eq it := ⟨Monadic.step it, rfl⟩
 
 theorem Iterator.Monadic.isPlausibleIndirectOutput_iff
     [UpwardEnumerable α] [LT α] [DecidableLT α] [LawfulUpwardEnumerableLT α]
@@ -1060,24 +1024,24 @@ loop implementation.
 @[always_inline, inline]
 instance Iterator.instIteratorLoop [UpwardEnumerable α] [LT α] [DecidableLT α]
     [LawfulUpwardEnumerable α] [LawfulUpwardEnumerableLT α]
-    {n : Type u → Type w} [Monad n] [MonadAttach n] :
+    {n : Type u → Type w} [Monad n] :
     IteratorLoop (Rxo.Iterator α) Id n where
-  forIn _ γ it init f :=
+  forIn _ γ Pl it init f :=
     match it with
     | ⟨⟨some next, upperBound⟩⟩ =>
-      loop γ (UpwardEnumerable.LE next ·) (fun a b hab hna => ?hle) upperBound init next ?hle'' (fun a ha c => f a ?hf c)
+      loop γ Pl (UpwardEnumerable.LE next ·) (fun a b hab hna => ?hle) upperBound init next ?hle'' (fun a ha₁ ha₂ c => f a ?hf c)
     | ⟨⟨none, _⟩⟩ => return init
   where
     @[always_inline, inline]
-    loop γ (LargeEnough : α → Prop)
+    loop γ (Pl : α → γ → ForInStep γ → Prop) (LargeEnough : α → Prop)
         (hl : ∀ a b : α, UpwardEnumerable.LE a b → LargeEnough a → LargeEnough b)
         (upperBound : α) (acc : γ) (next : α) (h : LargeEnough next)
-        (f : (out : α) → LargeEnough out ∧ out < upperBound → (c : γ) → n (ForInStep γ)) : n γ :=
+        (f : (out : α) → LargeEnough out → out < upperBound → (c : γ) → n (Subtype (Pl out c))) : n γ :=
       haveI : Nonempty γ := ⟨acc⟩
-      WellFounded.extrinsicFix₃ (C₃ := fun _ _ _ => n γ) (InvImage (IteratorLoop.rel _ Id (fun out h c => MonadAttach.CanReturn <| f out h c)) (fun x => (⟨Rxo.Iterator.mk (some x.1) upperBound⟩, x.2.1)))
+      WellFounded.extrinsicFix₃ (C₃ := fun _ _ _ => n γ) (InvImage (IteratorLoop.rel _ Id Pl) (fun x => (⟨Rxo.Iterator.mk (some x.1) upperBound⟩, x.2.1)))
         (fun next acc (h : LargeEnough next) G => do
           if hu : next < upperBound then
-            match ← MonadAttach.attach (f next ⟨h, hu⟩ acc) with
+            match ← f next h hu acc with
             | ⟨.yield acc', h'⟩ =>
               match hs : UpwardEnumerable.succ? next with
               | some next' => G next' acc' (hl _ _ ?hle' h) ?decreasing
@@ -1088,8 +1052,8 @@ instance Iterator.instIteratorLoop [UpwardEnumerable α] [LT α] [DecidableLT α
   finally
     case hf =>
       rw [Monadic.isPlausibleIndirectOutput_iff]
-      obtain ⟨n, hn⟩ := ha.1
-      exact ⟨n, hn, ha.2⟩
+      obtain ⟨n, hn⟩ := ha₁
+      exact ⟨n, hn, ha₂⟩
     case hle =>
       exact UpwardEnumerable.le_trans hna hab
     case hle' =>
@@ -1102,18 +1066,19 @@ instance Iterator.instIteratorLoop [UpwardEnumerable α] [LT α] [DecidableLT α
 
 private noncomputable def Iterator.instIteratorLoop.loop.wf [UpwardEnumerable α] [LT α] [DecidableLT α]
     [LawfulUpwardEnumerable α] [LawfulUpwardEnumerableLT α]
-    {n : Type u → Type w} [Monad n] [MonadAttach n] (γ : Type u)
+    {n : Type u → Type w} [Monad n] (γ : Type u)
+    (Pl : α → γ → ForInStep γ → Prop)
+    (wf : IteratorLoop.WellFounded (Rxo.Iterator α) Id Pl)
     (LargeEnough : α → Prop) (hl : ∀ a b : α, UpwardEnumerable.LE a b → LargeEnough a → LargeEnough b)
     (upperBound : α) (acc : γ) (next : α) (h : LargeEnough next)
-    (f : (out : α) → LargeEnough out ∧ out < upperBound → (c : γ) → n (ForInStep γ))
-    (wf : IteratorLoop.WellFounded (Rxo.Iterator α) Id (fun out h c => MonadAttach.CanReturn <| f out h c)) :
+    (f : (out : α) → LargeEnough out → out < upperBound → (c : γ) → n (Subtype (fun s : ForInStep γ => Pl out c s))) :
     n γ := do
   if hu : next < upperBound then
-    match ← MonadAttach.attach (f next ⟨h, hu⟩ acc) with
+    match ← f next h hu acc with
     | ⟨.yield acc', _⟩ =>
       match hs : UpwardEnumerable.succ? next with
       | some next' =>
-        loop.wf γ LargeEnough hl upperBound acc' next' (hl _ _ ?hle h) f wf
+        loop.wf γ Pl wf LargeEnough hl upperBound acc' next' (hl _ _ ?hle h) f
       | none => return acc'
     | ⟨.done acc', _⟩ => return acc'
   else
@@ -1127,14 +1092,14 @@ where finally
     simpa [succMany?_one] using hs
 
 private theorem Iterator.instIteratorLoop.loop_eq_wf [UpwardEnumerable α] [LT α] [DecidableLT α]
-    [LawfulUpwardEnumerable α] [LawfulUpwardEnumerableLT α] [Monad n] [MonadAttach n] [LawfulMonad n]
-    {γ LargeEnough hl upperBound} {next hn} {acc} (f wf) :
-    loop γ LargeEnough hl upperBound acc next hn f =
-      loop.wf (α := α) (n := n) γ LargeEnough hl upperBound acc next hn f wf := by
+    [LawfulUpwardEnumerable α] [LawfulUpwardEnumerableLT α] [Monad n] [LawfulMonad n]
+    {γ LargeEnough hl upperBound} {next hn} {acc} (Pl wf f) :
+    loop γ Pl LargeEnough hl upperBound acc next hn f =
+      loop.wf (α := α) (n := n) γ Pl wf LargeEnough hl upperBound acc next hn f := by
   haveI : Nonempty γ := ⟨acc⟩
   rw [loop, WellFounded.extrinsicFix₃_eq_fix]; rotate_left
   · exact InvImage.wf _ wf
-  · fun_induction loop.wf γ LargeEnough hl upperBound acc  next hn f wf
+  · fun_induction loop.wf γ Pl wf LargeEnough hl upperBound acc  next hn f
     · rw [WellFounded.fix_eq]
       simp only [↓reduceDIte, *]
       apply bind_congr; intro forInStep
@@ -1149,84 +1114,76 @@ private theorem Iterator.instIteratorLoop.loop_eq_wf [UpwardEnumerable α] [LT �
 
 private theorem Iterator.instIteratorLoop.loopWf_eq [UpwardEnumerable α] [LT α] [DecidableLT α]
     [LawfulUpwardEnumerable α] [LawfulUpwardEnumerableLT α]
-    {n : Type u → Type w} [Monad n] [MonadAttach n] [LawfulMonad n] [LawfulMonadAttach n]
-    (γ : Type u) {lift}
-    [instLawfulMonadLiftFunction : Std.Internal.LawfulMonadLiftBindFunction (m := Id) (n := n) lift]
+    {n : Type u → Type w} [Monad n] [LawfulMonad n] (γ : Type u)
+    {lift} [instLawfulMonadLiftFunction : Std.Internal.LawfulMonadLiftBindFunction (m := Id) (n := n) lift]
+    (Pl : α → γ → ForInStep γ → Prop)
+    (wf : IteratorLoop.WellFounded (Rxo.Iterator α) Id Pl)
     (LargeEnough : α → Prop) (hl : ∀ a b : α, UpwardEnumerable.LE a b → LargeEnough a → LargeEnough b)
     (upperBound : α) (acc : γ) (next : α) (h : LargeEnough next)
-    (f : (out : α) → LargeEnough out ∧ out < upperBound → (c : γ) → n (ForInStep γ))
-    (wf : IteratorLoop.WellFounded (Rxo.Iterator α) Id _) :
-    loop.wf γ LargeEnough hl upperBound acc next h f wf = (do
+    (f : (out : α) → LargeEnough out → out < upperBound → (c : γ) → n (Subtype (fun s : ForInStep γ => Pl out c s))) :
+    loop.wf γ Pl wf LargeEnough hl upperBound acc next h f = (do
       if hu : next < upperBound then
-        match ← MonadAttach.attach (f next ⟨h, hu⟩ acc) with
+        match ← f next h hu acc with
         | ⟨.yield acc', _⟩ =>
           letI it' : IterM (α := Rxo.Iterator α) Id α := ⟨⟨succ? next, upperBound⟩⟩
-          IterM.DefaultConsumers.forIn' (m := Id) (n := n) lift γ it' acc'
-            (fun a => LargeEnough a ∧ a < upperBound) (fun a h => by
-              rw [Monadic.isPlausibleIndirectOutput_iff] at h
-              obtain ⟨n, h₁, h₂⟩ := h
-              apply And.intro
-              · apply hl next a _ h
-                simp only [it', ← UpwardEnumerable.succMany?_add_one_eq_succ?_bind_succMany?] at h₁
-                exact ⟨n + 1, h₁⟩
-              · exact h₂)
-            fun next' h acc' => f next' h acc'
+          IterM.DefaultConsumers.forIn' (m := Id) (n := n) lift γ Pl it' acc'
+            it'.IsPlausibleIndirectOutput (fun _ => id)
+            fun next' h acc' => f next'
+              (by
+                refine hl next next' ?_ ‹_›
+                simp only [it', Monadic.isPlausibleIndirectOutput_iff,
+                  ← succMany?_add_one_eq_succ?_bind_succMany?] at h
+                exact ⟨h.choose + 1, h.choose_spec.1⟩)
+              (by
+                simp only [it', Monadic.isPlausibleIndirectOutput_iff] at h
+                exact h.choose_spec.2)
+              acc'
         | ⟨.done acc', _⟩ => return acc'
       else return acc) := by
-  fun_induction loop.wf γ LargeEnough hl upperBound acc next h f wf
-  · rename_i ih
-    simp only [↓reduceDIte, *]
-    apply bind_congr; intro forInStep
-    split
-    · split
-      · rw [ih _ ‹_› _ ‹_›]
-        rw [IterM.DefaultConsumers.forIn'_eq_match_step (lift := lift) (wf := wf)]; rotate_left
-        · simp only [Monadic.step_eq_step, MonadAttach.CanReturn, MonadAttach.attach, Monadic.step,
-            instLawfulMonadLiftFunction.liftBind_pure, *]
+  haveI : Nonempty γ := ⟨acc⟩
+  rw [loop.wf]
+  congr 1; ext hu
+  apply bind_congr; intro forInStep
+  split
+  · split
+    · rw [loopWf_eq (lift := lift) _ Pl wf]
+      rw [IterM.DefaultConsumers.forIn'_eq_match_step (lift := lift) Pl wf]; rotate_left
+      · simp only [Monadic.step_eq_step, Monadic.step,
+          Shrink.inflate_deflate, instLawfulMonadLiftFunction.liftBind_pure, *]
+        split
+        · apply bind_congr; intro forInStep
           split
-          · conv => rhs; simp only [Id.run_pure, ← LawfulMonadAttach.map_attach (x := f _ _ _),
-              bind_map_left]
-            apply bind_congr; intro forInStep
-            split
-            · apply IterM.DefaultConsumers.forIn'_eq_forIn' (wf := wf) (wf' := wf)
-              intros; simp
-            · simp
+          · apply IterM.DefaultConsumers.forIn'_eq_forIn' Pl wf <;> (intros; rfl)
           · simp
-      · rw [IterM.DefaultConsumers.forIn'_eq_match_step wf]
-        simp [MonadAttach.CanReturn, MonadAttach.attach, Monadic.step_eq_step, Monadic.step,
-          instLawfulMonadLiftFunction.liftBind_pure, *]
-    · simp
-  · simp only [right_eq_dite_iff]
-    intro h
-    exact Not.elim ‹_› h
+        · simp
+    · rw [IterM.DefaultConsumers.forIn'_eq_match_step Pl wf]
+      simp [Monadic.step_eq_step, Monadic.step, instLawfulMonadLiftFunction.liftBind_pure, *]
+  · simp
+termination_by IteratorLoop.WithWF.mk ⟨⟨some next, upperBound⟩⟩ acc (hwf := wf)
+decreasing_by
+  simp [IteratorLoop.rel, Monadic.isPlausibleStep_iff, Monadic.step, *]
 
 instance Iterator.instLawfulIteratorLoop [UpwardEnumerable α] [LT α] [DecidableLT α]
     [LawfulUpwardEnumerable α] [LawfulUpwardEnumerableLT α]
-    {n : Type u → Type w} [Monad n] [MonadAttach n] [LawfulMonad n] [LawfulMonadAttach n] :
+    {n : Type u → Type w} [Monad n] [LawfulMonad n] :
     LawfulIteratorLoop (Rxo.Iterator α) Id n where
   lawful := by
-    intro lift instLawfulMonadLiftFunction γ it init f wf
+    intro lift instLawfulMonadLiftFunction γ it init Pl wf f
     simp only [IteratorLoop.defaultImplementation, IteratorLoop.forIn,
-      IterM.DefaultConsumers.forIn'_eq_wf f wf]
+      IterM.DefaultConsumers.forIn'_eq_wf Pl wf]
     rw [IterM.DefaultConsumers.forIn'.wf]
     split; rotate_left
-    · simp [Monadic.step_eq_step, MonadAttach.CanReturn, MonadAttach.attach, Monadic.step,
-        Internal.LawfulMonadLiftBindFunction.liftBind_pure]
-    rename_i lo next f
-    have wf' := wf
-    rw [IteratorLoop.wellFounded_congr (Q := fun b => UpwardEnumerable.LE lo b ∧ b < next)] at wf'; rotate_left
-    · ext
-      simp [Monadic.isPlausibleIndirectOutput_iff, ← UpwardEnumerable.le_iff_exists]
-    rw [instIteratorLoop.loop_eq_wf (wf := wf'), instIteratorLoop.loopWf_eq (lift := lift)]; rotate_left
-    simp only [Monadic.step_eq_step, MonadAttach.CanReturn, MonadAttach.attach, Monadic.step,
-      instLawfulMonadLiftFunction.liftBind_pure]
+    · simp [Monadic.step_eq_step, Monadic.step, Internal.LawfulMonadLiftBindFunction.liftBind_pure]
+    rename_i next _
+    rw [instIteratorLoop.loop_eq_wf Pl wf, instIteratorLoop.loopWf_eq (lift := lift)]
+    simp only [Monadic.step_eq_step, Monadic.step, instLawfulMonadLiftFunction.liftBind_pure,
+      Shrink.inflate_deflate]
     split
     · apply bind_congr; intro forInStep
       split
       · simp only
-        rw [← IterM.DefaultConsumers.forIn'_eq_wf _ wf]
-        apply IterM.DefaultConsumers.forIn'_eq_forIn' wf' wf
-        intros; rfl
+        rw [← IterM.DefaultConsumers.forIn'_eq_wf Pl wf _]
+        apply IterM.DefaultConsumers.forIn'_eq_forIn' Pl wf <;> all_goals (intros; rfl)
       · simp
     · simp
 
@@ -1277,16 +1234,17 @@ theorem Iterator.step_eq_monadicStep [UpwardEnumerable α]
 @[always_inline, inline]
 instance [UpwardEnumerable α] :
     Iterator (Rxi.Iterator α) Id α where
-  step it := pure (Iterator.Monadic.step it)
+  IsPlausibleStep it step := step = Iterator.Monadic.step it
+  step it := pure (.deflate ⟨Iterator.Monadic.step it, rfl⟩)
 
 theorem Iterator.Monadic.isPlausibleStep_iff [UpwardEnumerable α]
     {it : IterM (α := Rxi.Iterator α) Id α} {step} :
     it.IsPlausibleStep step ↔ step = Iterator.Monadic.step it := by
-  simp [IterM.IsPlausibleStep, MonadAttach.CanReturn, Iterators.Iterator.step, eq_comm]
+  exact Iff.rfl
 
 theorem Iterator.Monadic.step_eq_step [UpwardEnumerable α]
     {it : IterM (α := Rxi.Iterator α) Id α} :
-    it.step = pure (Iterator.Monadic.step it) := by
+    it.step = pure (.deflate ⟨Iterator.Monadic.step it, isPlausibleStep_iff.mpr rfl⟩) := by
   simp [IterM.step, Iterators.Iterator.step]
 
 theorem Iterator.isPlausibleStep_iff [UpwardEnumerable α]
@@ -1304,7 +1262,7 @@ theorem Iterator.isPlausibleStep_iff [UpwardEnumerable α]
 
 theorem Iterator.step_eq_step [UpwardEnumerable α]
     {it : Iter (α := Rxi.Iterator α) α} :
-    it.step = Iterator.step it := by
+    it.step = ⟨Iterator.step it, isPlausibleStep_iff.mpr rfl⟩ := by
   simp [Iter.step, step_eq_monadicStep, Monadic.step_eq_step, IterM.Step.toPure]
 
 instance Iterator.instIteratorCollect [UpwardEnumerable α]
@@ -1349,14 +1307,15 @@ theorem Iterator.Monadic.isPlausibleSuccessorOf_iff
   constructor
   · rintro ⟨step, h, h'⟩
     cases h'
-    simp only [Iterators.Iterator.step, Monadic.step, Id.run_pure] at h
+    simp only [Monadic.step] at h
     split at h
     · cases h
     · cases h
       simp_all
   · rintro ⟨a, h, h'⟩
     refine ⟨.yield it' a, rfl, ?_⟩
-    simp only [IterM.IsPlausibleStep, MonadAttach.CanReturn, Iterators.Iterator.step, step, h]
+    simp only [IterM.IsPlausibleStep, Iterator.IsPlausibleStep, step, h,
+      IterStep.yield.injEq, and_true]
     simp [h']
 
 theorem Iterator.isPlausibleSuccessorOf_iff
@@ -1391,20 +1350,16 @@ private def Iterator.instFinitenessRelation [UpwardEnumerable α]
         ⟨⟨none⟩⟩ := by
       constructor
       intro it' ⟨step, hs₁, hs₂⟩
-      simp only [IterM.IsPlausibleStep, MonadAttach.CanReturn, Iterators.Iterator.step,
-        Monadic.step, Id.run_pure] at hs₂
-      simp [← hs₂, IterStep.successor] at hs₁
-    simp only [IterM.IsPlausibleSuccessorOf, IterM.IsPlausibleStep, MonadAttach.CanReturn,
-      Iterators.Iterator.step, Monadic.step] at hnone ⊢
+      simp only [IterM.IsPlausibleStep, Iterator.IsPlausibleStep, Monadic.step] at hs₂
+      simp [hs₂, IterStep.successor] at hs₁
+    simp only [IterM.IsPlausibleSuccessorOf, IterM.IsPlausibleStep, Iterator.IsPlausibleStep,
+      Monadic.step, exists_eq_right] at hnone ⊢
     match it with
     | ⟨⟨none⟩⟩ => apply hnone
     | ⟨⟨some init⟩⟩ =>
       obtain ⟨n, hn⟩ := Rxi.IsAlwaysFinite.finite init
       induction n generalizing init with
-      | zero =>
-        simp only [succMany?_zero] at hn
-        constructor
-        cases hn
+      | zero => simp [succMany?_zero] at hn
       | succ n ih =>
         constructor
         rintro it'
@@ -1413,14 +1368,12 @@ private def Iterator.instFinitenessRelation [UpwardEnumerable α]
         | none =>
           simp only [hs]
           intro h
-          obtain ⟨_, h, rfl⟩ := h
           cases h
           apply hnone
         | some a =>
           intro h
           simp only [hs] at h hn
           specialize ih _ hn
-          obtain ⟨_, h, rfl⟩ := h
           cases h
           exact ih
   subrelation := id
@@ -1438,8 +1391,8 @@ private def Iterator.instProductivenessRelation [UpwardEnumerable α]
   wf := emptyWf.wf
   subrelation {it it'} h := by
     exfalso
-    simp only [IterM.IsPlausibleSkipSuccessorOf, IterM.IsPlausibleStep, MonadAttach.CanReturn,
-      Iterators.Iterator.step, Monadic.step] at h
+    simp only [IterM.IsPlausibleSkipSuccessorOf, IterM.IsPlausibleStep,
+      Iterator.IsPlausibleStep, Monadic.step] at h
     split at h <;> cases h
 
 @[no_expose]
@@ -1451,16 +1404,10 @@ instance Iterator.instProductive [UpwardEnumerable α]
 instance Iterator.instIteratorAccess [UpwardEnumerable α]
     [LawfulUpwardEnumerable α] :
     IteratorAccess (Rxi.Iterator α) Id where
-  nextAtIdx? it n := match it.internalState.next.bind (UpwardEnumerable.succMany? n) with
+  nextAtIdx? it n := ⟨match it.internalState.next.bind (UpwardEnumerable.succMany? n) with
     | none => .done
-    | some next => .yield ⟨⟨UpwardEnumerable.succ? next⟩⟩ next
-
-instance Iterator.instLawfulIteratorAccess [UpwardEnumerable α]
-    [LawfulUpwardEnumerable α] :
-    LawfulIteratorAccess (Rxi.Iterator α) Id where
-  isPlausibleNthOutputStep_of_canReturn {it n s} h := by
-      simp only [MonadAttach.CanReturn, IteratorAccess.nextAtIdx?] at h
-      cases h
+    | some next =>
+        .yield ⟨⟨UpwardEnumerable.succ? next⟩⟩ next, (by
       induction n generalizing it
       · split <;> rename_i heq
         · apply IterM.IsPlausibleNthOutputStep.done
@@ -1476,8 +1423,8 @@ instance Iterator.instLawfulIteratorAccess [UpwardEnumerable α]
           · simp [heq'] at heq
           simp only [heq', Option.bind_some, succMany?_zero, Option.some.injEq] at heq
           cases heq
-          apply IterM.IsPlausibleNthOutputStep.zero_yield
-          simp [Monadic.isPlausibleStep_iff, Monadic.step, heq']
+          · apply IterM.IsPlausibleNthOutputStep.zero_yield
+            simp [Monadic.isPlausibleStep_iff, Monadic.step, heq']
       · rename_i n ih
         split <;> rename_i heq
         · cases heq' : it.internalState.next
@@ -1485,30 +1432,30 @@ instance Iterator.instLawfulIteratorAccess [UpwardEnumerable α]
             simp only [Monadic.isPlausibleStep_iff, Monadic.step, heq']
           · rename_i out
             simp only [heq', Option.bind_some, succMany?_add_one_eq_succ?_bind_succMany?] at heq
-            specialize ih (it := ⟨⟨UpwardEnumerable.succ? out⟩⟩)
+            specialize ih ⟨⟨UpwardEnumerable.succ? out⟩⟩
             simp only [heq] at ih
-            apply IterM.IsPlausibleNthOutputStep.yield
-            · simp only [Monadic.isPlausibleStep_iff, Monadic.step, heq',
-              IterStep.yield.injEq]
-              exact ⟨rfl, rfl⟩
-            · exact ih
+            · apply IterM.IsPlausibleNthOutputStep.yield
+              · simp only [Monadic.isPlausibleStep_iff, Monadic.step, heq',
+                IterStep.yield.injEq]
+                exact ⟨rfl, rfl⟩
+              · exact ih
         · cases heq' : it.internalState.next
           · simp [heq'] at heq
           rename_i out
           simp only [heq', Option.bind_some] at heq
           have hlt : UpwardEnumerable.LT out _ := ⟨n, heq⟩
           simp only [succMany?_add_one_eq_succ?_bind_succMany?] at heq
-          specialize ih (it := ⟨⟨UpwardEnumerable.succ? out⟩⟩)
+          specialize ih ⟨⟨UpwardEnumerable.succ? out⟩⟩
           simp only [heq] at ih
           · apply IterM.IsPlausibleNthOutputStep.yield
-            · simp only [Monadic.isPlausibleStep_iff, Monadic.step, heq', IterStep.yield.injEq]
+            · simp only [Monadic.isPlausibleStep_iff, Monadic.step, heq',
+              IterStep.yield.injEq]
               exact ⟨rfl, rfl⟩
-            · apply ih
+            · apply ih)⟩
 
 instance Iterator.instLawfulDeterministicIterator [UpwardEnumerable α] :
     LawfulDeterministicIterator (Rxi.Iterator α) Id where
-  isPlausibleStep_eq_eq it := ⟨Monadic.step it, by
-      simp [IterM.IsPlausibleStep, MonadAttach.CanReturn, Iterators.Iterator.step, eq_comm]⟩
+  isPlausibleStep_eq_eq it := ⟨Monadic.step it, rfl⟩
 
 theorem Iterator.Monadic.isPlausibleIndirectOutput_iff
     [UpwardEnumerable α] [LawfulUpwardEnumerable α]
@@ -1566,22 +1513,22 @@ loop implementation.
 -/
 @[always_inline, inline]
 instance Iterator.instIteratorLoop [UpwardEnumerable α] [LawfulUpwardEnumerable α]
-    {n : Type u → Type w} [Monad n] [MonadAttach n] :
+    {n : Type u → Type w} [Monad n] :
     IteratorLoop (Rxi.Iterator α) Id n where
-  forIn _ γ it init f :=
+  forIn _ γ Pl it init f :=
     match it with
     | ⟨⟨some next⟩⟩ =>
-      loop γ (UpwardEnumerable.LE next ·) (fun a b hab hna => ?hle) init next ?hle'' (fun a ha c => f a ?hf c)
+      loop γ Pl (UpwardEnumerable.LE next ·) (fun a b hab hna => ?hle) init next ?hle'' (fun a ha c => f a ?hf c)
     | ⟨⟨none⟩⟩ => return init
   where
     @[always_inline, inline]
-    loop γ (LargeEnough : α → Prop) (hl : ∀ a b : α, UpwardEnumerable.LE a b → LargeEnough a → LargeEnough b)
+    loop γ (Pl : α → γ → ForInStep γ → Prop) (LargeEnough : α → Prop) (hl : ∀ a b : α, UpwardEnumerable.LE a b → LargeEnough a → LargeEnough b)
         (acc : γ) (next : α) (h : LargeEnough next)
-        (f : (out : α) → LargeEnough out → (c : γ) → n (ForInStep γ)) : n γ :=
+        (f : (out : α) → LargeEnough out → (c : γ) → n (Subtype (Pl out c))) : n γ :=
       haveI : Nonempty γ := ⟨acc⟩
-      WellFounded.extrinsicFix₃ (C₃ := fun _ _ _ => n γ) (InvImage (IteratorLoop.rel _ Id (fun out h c => MonadAttach.CanReturn <| f out h c)) (fun x => (⟨Rxi.Iterator.mk (some x.1)⟩, x.2.1)))
+      WellFounded.extrinsicFix₃ (C₃ := fun _ _ _ => n γ) (InvImage (IteratorLoop.rel _ Id Pl) (fun x => (⟨Rxi.Iterator.mk (some x.1)⟩, x.2.1)))
         (fun next acc (h : LargeEnough next) G => do
-          match ← MonadAttach.attach (f next h acc) with
+          match ← f next h acc with
           | ⟨.yield acc', h'⟩ =>
             match hs : UpwardEnumerable.succ? next with
             | some next' => G next' acc' (hl _ _ ?hle' h) ?decreasing
@@ -1603,17 +1550,18 @@ instance Iterator.instIteratorLoop [UpwardEnumerable α] [LawfulUpwardEnumerable
 
 private noncomputable def Iterator.instIteratorLoop.loop.wf [UpwardEnumerable α]
     [LawfulUpwardEnumerable α]
-    {n : Type u → Type w} [Monad n] [MonadAttach n] (γ : Type u)
+    {n : Type u → Type w} [Monad n] (γ : Type u)
+    (Pl : α → γ → ForInStep γ → Prop)
+    (wf : IteratorLoop.WellFounded (Rxi.Iterator α) Id Pl)
     (LargeEnough : α → Prop) (hl : ∀ a b : α, UpwardEnumerable.LE a b → LargeEnough a → LargeEnough b)
     (acc : γ) (next : α) (h : LargeEnough next)
-    (f : (out : α) → LargeEnough out → (c : γ) → n (ForInStep γ))
-    (wf : IteratorLoop.WellFounded (Rxi.Iterator α) Id (fun out h c => MonadAttach.CanReturn <| f out h c)) :
+    (f : (out : α) → LargeEnough out → (c : γ) → n (Subtype (fun s : ForInStep γ => Pl out c s))) :
     n γ := do
-    match ← MonadAttach.attach (f next h acc) with
+    match ← f next h acc with
     | ⟨.yield acc', _⟩ =>
       match hs : UpwardEnumerable.succ? next with
       | some next' =>
-        loop.wf γ LargeEnough hl acc' next' (hl _ _ ?hle h) f wf
+        loop.wf γ Pl wf LargeEnough hl acc' next' (hl _ _ ?hle h) f
       | none => return acc'
     | ⟨.done acc', _⟩ => return acc'
 termination_by IteratorLoop.WithWF.mk ⟨⟨some next⟩⟩ acc (hwf := wf)
@@ -1625,14 +1573,14 @@ where finally
     simpa [succMany?_one] using hs
 
 private theorem Iterator.instIteratorLoop.loop_eq_wf [UpwardEnumerable α]
-    [LawfulUpwardEnumerable α] [Monad n] [MonadAttach n] [LawfulMonad n]
-    {γ LargeEnough hl} {next hn} {acc} (f wf) :
-    loop γ LargeEnough hl acc next hn f =
-      loop.wf (α := α) (n := n) γ LargeEnough hl acc next hn f wf := by
+    [LawfulUpwardEnumerable α] [Monad n] [LawfulMonad n]
+    {γ LargeEnough hl} {next hn} {acc} (Pl wf f) :
+    loop γ Pl LargeEnough hl acc next hn f =
+      loop.wf (α := α) (n := n) γ Pl wf LargeEnough hl acc next hn f := by
   haveI : Nonempty γ := ⟨acc⟩
   rw [loop, WellFounded.extrinsicFix₃_eq_fix]; rotate_left
   · exact InvImage.wf _ wf
-  · fun_induction loop.wf γ LargeEnough hl acc  next hn f wf
+  · fun_induction loop.wf γ Pl wf LargeEnough hl acc  next hn f
     · rw [WellFounded.fix_eq]
       apply bind_congr; intro forInStep
       split
@@ -1644,72 +1592,67 @@ private theorem Iterator.instIteratorLoop.loop_eq_wf [UpwardEnumerable α]
 
 private theorem Iterator.instIteratorLoop.loopWf_eq [UpwardEnumerable α]
     [LawfulUpwardEnumerable α]
-    {n : Type u → Type w} [Monad n] [MonadAttach n] [LawfulMonad n] [LawfulMonadAttach n] (γ : Type u)
+    {n : Type u → Type w} [Monad n] [LawfulMonad n] (γ : Type u)
     {lift} [instLawfulMonadLiftFunction : Std.Internal.LawfulMonadLiftBindFunction (m := Id) (n := n) lift]
+    (Pl : α → γ → ForInStep γ → Prop)
+    (wf : IteratorLoop.WellFounded (Rxi.Iterator α) Id Pl)
     (LargeEnough : α → Prop) (hl : ∀ a b : α, UpwardEnumerable.LE a b → LargeEnough a → LargeEnough b)
     (acc : γ) (next : α) (h : LargeEnough next)
-    (f : (out : α) → LargeEnough out → (c : γ) → n (ForInStep γ))
-    (wf : IteratorLoop.WellFounded (Rxi.Iterator α) Id _) :
-    loop.wf γ LargeEnough hl acc next h f wf = (do
-        match ← MonadAttach.attach (f next h acc) with
+    (f : (out : α) → LargeEnough out → (c : γ) → n (Subtype (fun s : ForInStep γ => Pl out c s))) :
+    loop.wf γ Pl wf LargeEnough hl acc next h f = (do
+        match ← f next h acc with
         | ⟨.yield acc', _⟩ =>
           letI it' : IterM (α := Rxi.Iterator α) Id α := ⟨⟨succ? next⟩⟩
-          IterM.DefaultConsumers.forIn' (m := Id) (n := n) lift γ it' acc'
-            LargeEnough (fun a h => by
-              rw [Monadic.isPlausibleIndirectOutput_iff] at h
-              apply hl next a _ ‹_›
-              obtain ⟨n, h⟩ := h
-              simp only [it', ← succMany?_add_one_eq_succ?_bind_succMany?] at h
-              exact ⟨n + 1, h⟩)
-            fun next' h acc' => f next' h acc'
+          IterM.DefaultConsumers.forIn' (m := Id) (n := n) lift γ Pl it' acc'
+            it'.IsPlausibleIndirectOutput (fun _ => id)
+            fun next' h acc' => f next'
+              (by
+                refine hl next next' ?_ ‹_›
+                simp only [it', Monadic.isPlausibleIndirectOutput_iff,
+                  ← succMany?_add_one_eq_succ?_bind_succMany?] at h
+                exact ⟨h.choose + 1, h.choose_spec⟩)
+              acc'
         | ⟨.done acc', _⟩ => return acc') := by
-  fun_induction loop.wf γ LargeEnough hl acc next h f wf
-  · rename_i ih
-    apply bind_congr; intro forInStep
-    split
-    · split
-      · rw [ih _ ‹_› _ ‹_›]
-        rw [IterM.DefaultConsumers.forIn'_eq_match_step (lift := lift) (wf := wf)]; rotate_left
-        · simp only [Monadic.step_eq_step, MonadAttach.CanReturn, MonadAttach.attach, Monadic.step,
-            instLawfulMonadLiftFunction.liftBind_pure, Id.run_pure, *]
-          conv => rhs; simp only [Id.run_pure, ← LawfulMonadAttach.map_attach (x := f _ _ _),
-            bind_map_left]
-          apply bind_congr; intro forInStep
-          split
-          · apply IterM.DefaultConsumers.forIn'_eq_forIn' (wf := wf) (wf' := wf)
-            intros; simp
-          · simp
-      · rw [IterM.DefaultConsumers.forIn'_eq_match_step wf]
-        simp [MonadAttach.CanReturn, MonadAttach.attach, Monadic.step_eq_step, Monadic.step,
-          instLawfulMonadLiftFunction.liftBind_pure, *]
-    · simp
+  haveI : Nonempty γ := ⟨acc⟩
+  rw [loop.wf]
+  apply bind_congr; intro forInStep
+  split
+  · split
+    · rw [loopWf_eq (lift := lift) _ Pl wf]
+      rw [IterM.DefaultConsumers.forIn'_eq_match_step (lift := lift) Pl wf]; rotate_left
+      · simp only [Monadic.step_eq_step, Monadic.step,
+          Shrink.inflate_deflate, instLawfulMonadLiftFunction.liftBind_pure, *]
+        apply bind_congr; intro forInStep
+        split
+        · apply IterM.DefaultConsumers.forIn'_eq_forIn' Pl wf <;> (intros; rfl)
+        · simp
+    · rw [IterM.DefaultConsumers.forIn'_eq_match_step Pl wf]
+      simp [Monadic.step_eq_step, Monadic.step, instLawfulMonadLiftFunction.liftBind_pure, *]
+  · simp
+termination_by IteratorLoop.WithWF.mk ⟨⟨some next⟩⟩ acc (hwf := wf)
+decreasing_by
+  simp [IteratorLoop.rel, Monadic.isPlausibleStep_iff, Monadic.step, *]
 
 instance Iterator.instLawfulIteratorLoop [UpwardEnumerable α]
     [LawfulUpwardEnumerable α]
-    {n : Type u → Type w} [Monad n] [MonadAttach n] [LawfulMonad n] [LawfulMonadAttach n] :
+    {n : Type u → Type w} [Monad n] [LawfulMonad n] :
     LawfulIteratorLoop (Rxi.Iterator α) Id n where
   lawful := by
-    intro lift instLawfulMonadLiftFunction γ it init f wf
+    intro lift instLawfulMonadLiftFunction γ it init Pl wf f
     simp only [IteratorLoop.defaultImplementation, IteratorLoop.forIn,
-      IterM.DefaultConsumers.forIn'_eq_wf f wf]
+      IterM.DefaultConsumers.forIn'_eq_wf Pl wf]
     rw [IterM.DefaultConsumers.forIn'.wf]
     split; rotate_left
-    · simp [Monadic.step_eq_step, MonadAttach.CanReturn, MonadAttach.attach, Monadic.step,
-        Internal.LawfulMonadLiftBindFunction.liftBind_pure]
-    rename_i lo f
-    have wf' := wf
-    rw [IteratorLoop.wellFounded_congr (Q := fun b => UpwardEnumerable.LE lo b)] at wf'; rotate_left
-    · ext
-      simp [Monadic.isPlausibleIndirectOutput_iff, ← UpwardEnumerable.le_iff_exists]
-    rw [instIteratorLoop.loop_eq_wf (wf := wf'), instIteratorLoop.loopWf_eq (lift := lift)]; rotate_left
-    simp only [Monadic.step_eq_step, MonadAttach.CanReturn, MonadAttach.attach, Monadic.step,
-      instLawfulMonadLiftFunction.liftBind_pure, Id.run_pure]
+    · simp [Monadic.step_eq_step, Monadic.step, Internal.LawfulMonadLiftBindFunction.liftBind_pure]
+    rename_i next _
+    rw [instIteratorLoop.loop_eq_wf Pl wf, instIteratorLoop.loopWf_eq (lift := lift)]
+    simp only [Monadic.step_eq_step, Monadic.step, instLawfulMonadLiftFunction.liftBind_pure,
+      Shrink.inflate_deflate]
     apply bind_congr; intro forInStep
     split
     · simp only
-      rw [← IterM.DefaultConsumers.forIn'_eq_wf _ wf]
-      apply IterM.DefaultConsumers.forIn'_eq_forIn' wf' wf
-      intros; rfl
+      rw [← IterM.DefaultConsumers.forIn'_eq_wf Pl wf _]
+      apply IterM.DefaultConsumers.forIn'_eq_forIn' Pl wf <;> all_goals (intros; rfl)
     · simp
 
 end IteratorLoop
