src/Init/Data/Iterators/Combinators/Monadic/FilterMap.lean
@@ -9,7 +9,6 @@ prelude
 public import Init.Data.Iterators.Consumers.Loop
 public import Init.Data.Iterators.PostconditionMonad
 public import Init.Data.Iterators.Internal.Termination
-import Init.Control.Lawful.MonadAttach.Lemmas
 
 public section
 
@@ -41,7 +40,7 @@ Internal state of the `filterMap` combinator. Do not depend on its internals.
 @[ext, unbox]
 structure FilterMap (α : Type w) {β γ : Type w}
     (m : Type w → Type w') (n : Type w → Type w'') (lift : ⦃α : Type w⦄ → m α → n α)
-    (f : β → n (Option γ)) where
+    (f : β → PostconditionT n (Option γ)) where
   /-- Internal implementation detail of the iterator library. -/
   inner : IterM (α := α) m β
 
@@ -51,22 +50,301 @@ Internal state of the `map` combinator. Do not depend on its internals.
 @[expose]
 def Map (α : Type w) {β γ : Type w} (m : Type w → Type w') (n : Type w → Type w'')
     (lift : ⦃α : Type w⦄ → m α → n α) [Functor n]
-    (f : β → n γ) :=
-  FilterMap α m n lift (fun b => some <$> f b)
+    (f : β → PostconditionT n γ) :=
+  FilterMap α m n lift (fun b => PostconditionT.map some (f b))
 
 @[always_inline, inline, expose]
 def IterM.InternalCombinators.filterMap {α β γ : Type w} {m : Type w → Type w'}
     {n : Type w → Type w''} (lift : ⦃α : Type w⦄ → m α → n α)
-    [Iterator α m β] (f : β → n (Option γ))
+    [Iterator α m β] (f : β → PostconditionT n (Option γ))
     (it : IterM (α := α) m β) : IterM (α := FilterMap α m n lift f) n γ :=
   toIterM ⟨it⟩ n γ
 
 @[always_inline, inline, expose]
 def IterM.InternalCombinators.map {α β γ : Type w} {m : Type w → Type w'}
     {n : Type w → Type w''} [Monad n] (lift : ⦃α : Type w⦄ → m α → n α)
-    [Iterator α m β] (f : β → n γ)
+    [Iterator α m β] (f : β → PostconditionT n γ)
     (it : IterM (α := α) m β) : IterM (α := Map α m n lift f) n γ :=
   toIterM ⟨it⟩ n γ
+
+/--
+*Note: This is a very general combinator that requires an advanced understanding of monads,
+dependent types and termination proofs. The variants `filterMap` and `filterMapM` are easier to use
+and sufficient for most use cases.*
+
+If `it` is an iterator, then `it.filterMapWithPostcondition f` is another iterator that applies a
+monadic function `f` to all values emitted by `it`. `f` is expected to return an `Option` inside the
+monad. If `f` returns `none`, then nothing is emitted; if it returns `some x`, then `x` is emitted.
+
+`f` is expected to return `PostconditionT n (Option _)`. The base iterator `it` being monadic in
+`m`, `n` can be different from `m`, but `it.filterMapWithPostcondition f` expects a `MonadLiftT m n`
+instance. The `PostconditionT` transformer allows the caller to intrinsically prove properties about
+`f`'s return value in the monad `n`, enabling termination proofs depending on the specific behavior
+of `f`.
+
+**Marble diagram (without monadic effects):**
+
+```text
+it                                ---a --b--c --d-e--⊥
+it.filterMapWithPostcondition     ---a'-----c'-------⊥
+```
+
+(given that `f a = pure (some a)'`, `f c = pure (some c')` and `f b = f d = d e = pure none`)
+
+**Termination properties:**
+
+* `Finite` instance: only if `it` is finite
+* `Productive` instance: only if `it` is finite
+
+For certain mapping functions `f`, the resulting iterator will be finite (or productive) even though
+no `Finite` (or `Productive`) instance is provided. For example, if `f` never returns `none`, then
+this combinator will preserve productiveness. If `f` is an `ExceptT` monad and will always fail,
+then `it.filterMapWithPostcondition` will be finite even if `it` isn't. In the first case, consider
+using the `map`/`mapM`/`mapWithPostcondition` combinators instead, which provide more instances out of
+the box.
+
+In such situations, the missing instances can be proved manually if the postcondition bundled in
+the `PostconditionT n` monad is strong enough. If `f` always returns `some _`, a suitable
+postcondition is `fun x => x.isSome`; if `f` always fails, a suitable postcondition might be
+`fun _ => False`.
+
+**Performance:**
+
+For each value emitted by the base iterator `it`, this combinator calls `f` and matches on the
+returned `Option` value.
+-/
+@[inline, expose]
+def IterM.filterMapWithPostcondition {α β γ : Type w} {m : Type w → Type w'} {n : Type w → Type w''}
+    [MonadLiftT m n] [Iterator α m β] (f : β → PostconditionT n (Option γ))
+    (it : IterM (α := α) m β) : IterM (α := FilterMap α m n (fun ⦃_⦄ => monadLift) f) n γ :=
+  IterM.InternalCombinators.filterMap (fun ⦃_⦄ => monadLift) f it
+
+/--
+`it.PlausibleStep step` is the proposition that `step` is a possible next step from the
+`filterMap` iterator `it`. This is mostly internally relevant, except if one needs to manually
+prove termination (`Finite` or `Productive` instances, for example) of a `filterMap` iterator.
+-/
+inductive FilterMap.PlausibleStep {α β γ : Type w} {m : Type w → Type w'} {n : Type w → Type w''}
+    {lift : ⦃α : Type w⦄ → m α → n α} {f : β → PostconditionT n (Option γ)} [Iterator α m β]
+    (it : IterM (α := FilterMap α m n lift f) n γ) :
+    IterStep (IterM (α := FilterMap α m n lift f) n γ) γ → Prop where
+  | yieldNone : ∀ {it' out},
+      it.internalState.inner.IsPlausibleStep (.yield it' out) →
+      (f out).Property none →
+      PlausibleStep it (.skip (IterM.InternalCombinators.filterMap lift f it'))
+  | yieldSome : ∀ {it' out out'}, it.internalState.inner.IsPlausibleStep (.yield it' out) →
+      (f out).Property (some out') →
+      PlausibleStep it (.yield (IterM.InternalCombinators.filterMap lift f it') out')
+  | skip : ∀ {it'}, it.internalState.inner.IsPlausibleStep (.skip it') →
+      PlausibleStep it (.skip (IterM.InternalCombinators.filterMap lift f it'))
+  | done : it.internalState.inner.IsPlausibleStep .done → PlausibleStep it .done
+
+instance FilterMap.instIterator {α β γ : Type w} {m : Type w → Type w'} {n : Type w → Type w''}
+    {lift : ⦃α : Type w⦄ → m α → n α} {f : β → PostconditionT n (Option γ)}
+    [Iterator α m β] [Monad n] :
+    Iterator (FilterMap α m n lift f) n γ where
+  IsPlausibleStep := FilterMap.PlausibleStep (m := m) (n := n)
+  step it :=
+    letI : MonadLift m n := ⟨lift (α := _)⟩
+    do
+      match (← it.internalState.inner.step).inflate with
+      | .yield it' out h => do
+        match ← (f out).operation with
+        | ⟨none, h'⟩ => pure <| .deflate <| .skip (it'.filterMapWithPostcondition f) (by exact .yieldNone h h')
+        | ⟨some out', h'⟩ => pure <| .deflate <| .yield (it'.filterMapWithPostcondition f) out' (by exact .yieldSome h h')
+      | .skip it' h => pure <| .deflate <| .skip (it'.filterMapWithPostcondition f) (by exact .skip h)
+      | .done h => pure <| .deflate <| .done (.done h)
+
+instance {α β γ : Type w} {m : Type w → Type w'} {n : Type w → Type w''} [Monad n] [Iterator α m β]
+    {lift : ⦃α : Type w⦄ → m α → n α}
+    {f : β → PostconditionT n γ} :
+    Iterator (Map α m n lift f) n γ :=
+  inferInstanceAs <| Iterator (FilterMap α m n lift _) n γ
+
+private def FilterMap.instFinitenessRelation {α β γ : Type w} {m : Type w → Type w'}
+    {n : Type w → Type w''} [Monad n] [Iterator α m β] {lift : ⦃α : Type w⦄ → m α → n α}
+    {f : β → PostconditionT n (Option γ)} [Finite α m] :
+    FinitenessRelation (FilterMap α m n lift f) n where
+  rel := InvImage IterM.IsPlausibleSuccessorOf (FilterMap.inner ∘ IterM.internalState)
+  wf := InvImage.wf _ Finite.wf
+  subrelation {it it'} h := by
+    obtain ⟨step, h, h'⟩ := h
+    cases h'
+    case yieldNone it' out h' h'' =>
+      cases h
+      exact IterM.isPlausibleSuccessorOf_of_yield h'
+    case yieldSome it' out h' h'' =>
+      cases h
+      exact IterM.isPlausibleSuccessorOf_of_yield h'
+    case skip it' h' =>
+      cases h
+      exact IterM.isPlausibleSuccessorOf_of_skip h'
+    case done h' =>
+      cases h
+
+@[no_expose]
+instance FilterMap.instFinite {α β γ : Type w} {m : Type w → Type w'}
+    {n : Type w → Type w''} [Monad n] [Iterator α m β] {lift : ⦃α : Type w⦄ → m α → n α}
+    {f : β → PostconditionT n (Option γ)} [Finite α m] : Finite (FilterMap α m n lift f) n :=
+  Finite.of_finitenessRelation FilterMap.instFinitenessRelation
+
+@[no_expose]
+instance {α β γ : Type w} {m : Type w → Type w'} {n : Type w → Type w''} [Monad n] [Iterator α m β]
+    {lift : ⦃α : Type w⦄ → m α → n α} {f : β → PostconditionT n γ} [Finite α m] :
+    Finite (Map α m n lift f) n :=
+  Finite.of_finitenessRelation FilterMap.instFinitenessRelation
+
+private def Map.instProductivenessRelation {α β γ : Type w} {m : Type w → Type w'}
+    {n : Type w → Type w''} [Monad n] [Iterator α m β] {lift : ⦃α : Type w⦄ → m α → n α}
+    {f : β → PostconditionT n γ} [Productive α m] :
+    ProductivenessRelation (Map α m n lift f) n where
+  rel := InvImage IterM.IsPlausibleSkipSuccessorOf (FilterMap.inner ∘ IterM.internalState)
+  wf := InvImage.wf _ Productive.wf
+  subrelation {it it'} h := by
+    cases h
+    case yieldNone it' out h h' =>
+      simp at h'
+    case skip it' h =>
+      exact h
+
+@[no_expose]
+instance Map.instProductive {α β γ : Type w} {m : Type w → Type w'}
+    {n : Type w → Type w''} [Monad n] [Iterator α m β] {lift : ⦃α : Type w⦄ → m α → n α}
+    {f : β → PostconditionT n γ} [Productive α m] :
+    Productive (Map α m n lift f) n :=
+  Productive.of_productivenessRelation Map.instProductivenessRelation
+
+instance {α β γ : Type w} {m : Type w → Type w'}
+    {n : Type w → Type w''} {o : Type w → Type x} [Monad n] [Monad o] [Iterator α m β]
+    {lift : ⦃α : Type w⦄ → m α → n α}
+    {f : β → PostconditionT n (Option γ)} :
+    IteratorCollect (FilterMap α m n lift f) n o :=
+  .defaultImplementation
+
+instance FilterMap.instIteratorLoop {α β γ : Type w} {m : Type w → Type w'}
+    {n : Type w → Type w''} {o : Type x → Type x'}
+    [Monad n] [Monad o] [Iterator α m β] {lift : ⦃α : Type w⦄ → m α → n α}
+    {f : β → PostconditionT n (Option γ)} :
+    IteratorLoop (FilterMap α m n lift f) n o :=
+  .defaultImplementation
+
+/--
+`map` operations allow for a more efficient implementation of `toArray`. For example,
+`array.iter.map f |>.toArray happens in-place if possible.
+-/
+instance Map.instIteratorCollect {α β γ : Type w} {m : Type w → Type w'}
+    {n : Type w → Type w''} {o : Type w → Type x} [Monad n] [Monad o] [Iterator α m β]
+    {lift₁ : ⦃α : Type w⦄ → m α → n α}
+    {f : β → PostconditionT n γ} [IteratorCollect α m o] :
+    IteratorCollect (Map α m n lift₁ f) n o where
+  toArrayMapped lift₂ _ g it :=
+    letI : MonadLift m n := ⟨lift₁ (α := _)⟩
+    letI : MonadLift n o := ⟨lift₂ (δ := _)⟩
+    IteratorCollect.toArrayMapped
+      (lift := fun ⦃_⦄ => monadLift)
+      (fun x => do g (← (f x).operation))
+      it.internalState.inner (m := m)
+
+instance Map.instIteratorLoop {α β γ : Type w} {m : Type w → Type w'}
+    {n : Type w → Type w''} {o : Type x → Type x'} [Monad n] [Monad o] [Iterator α m β]
+    {lift : ⦃α : Type w⦄ → m α → n α}
+    {f : β → PostconditionT n γ} :
+    IteratorLoop (Map α m n lift f) n o :=
+  .defaultImplementation
+
+/--
+*Note: This is a very general combinator that requires an advanced understanding of monads, dependent
+types and termination proofs. The variants `map` and `mapM` are easier to use and sufficient
+for most use cases.*
+
+If `it` is an iterator, then `it.mapWithPostcondition f` is another iterator that applies a monadic
+function `f` to all values emitted by `it` and emits the result.
+
+`f` is expected to return `PostconditionT n _`. The base iterator `it` being monadic in
+`m`, `n` can be different from `m`, but `it.mapWithPostcondition f` expects a `MonadLiftT m n`
+instance. The `PostconditionT` transformer allows the caller to intrinsically prove properties about
+`f`'s return value in the monad `n`, enabling termination proofs depending on the specific behavior
+of `f`.
+
+**Marble diagram (without monadic effects):**
+
+```text
+it                          ---a --b --c --d -e ----⊥
+it.mapWithPostcondition     ---a'--b'--c'--d'-e'----⊥
+```
+
+(given that `f a = pure a'`, `f b = pure b'` etc.)
+
+**Termination properties:**
+
+* `Finite` instance: only if `it` is finite
+* `Productive` instance: only if `it` is productive
+
+For certain mapping functions `f`, the resulting iterator will be finite (or productive) even though
+no `Finite` (or `Productive`) instance is provided. For example, if `f` is an `ExceptT` monad and
+will always fail, then `it.mapWithPostcondition` will be finite even if `it` isn't.
+
+In such situations, the missing instances can be proved manually if the postcondition bundled in
+the `PostconditionT n` monad is strong enough. In the given example, a suitable postcondition might
+be `fun _ => False`.
+
+**Performance:**
+
+For each value emitted by the base iterator `it`, this combinator calls `f`.
+-/
+@[inline, expose]
+def IterM.mapWithPostcondition {α β γ : Type w} {m : Type w → Type w'} {n : Type w → Type w''}
+    [Monad n] [MonadLiftT m n] [Iterator α m β] (f : β → PostconditionT n γ)
+    (it : IterM (α := α) m β) : IterM (α := Map α m n (fun ⦃_⦄ => monadLift) f) n γ :=
+  InternalCombinators.map (fun {_} => monadLift) f it
+
+/--
+*Note: This is a very general combinator that requires an advanced understanding of monads,
+dependent types and termination proofs. The variants `filter` and `filterM` are easier to use and
+sufficient for most use cases.*
+
+If `it` is an iterator, then `it.filterWithPostcondition f` is another iterator that applies a monadic
+predicate `f` to all values emitted by `it` and emits them only if they are accepted by `f`.
+
+`f` is expected to return `PostconditionT n (ULift Bool)`. The base iterator `it` being monadic in
+`m`, `n` can be different from `m`, but `it.filterWithPostcondition f` expects a `MonadLiftT m n`
+instance. The `PostconditionT` transformer allows the caller to intrinsically prove properties about
+`f`'s return value in the monad `n`, enabling termination proofs depending on the specific behavior
+of `f`.
+
+**Marble diagram (without monadic effects):**
+
+```text
+it                             ---a--b--c--d-e--⊥
+it.filterWithPostcondition     ---a-----c-------⊥
+```
+
+(given that `f a = f c = pure true` and `f b = f d = d e = pure false`)
+
+**Termination properties:**
+
+* `Finite` instance: only if `it` is finite
+* `Productive` instance: only if `it` is finite`
+
+For certain mapping functions `f`, the resulting iterator will be finite (or productive) even though
+no `Finite` (or `Productive`) instance is provided. For example, if `f` is an `ExceptT` monad and
+will always fail, then `it.filterWithPostcondition` will be finite -- and productive -- even if `it`
+isn't.
+
+In such situations, the missing instances can be proved manually if the postcondition bundled in
+the `PostconditionT n` monad is strong enough. In the given example, a suitable postcondition might
+be `fun _ => False`.
+
+**Performance:**
+
+For each value emitted by the base iterator `it`, this combinator calls `f`.
+-/
+@[inline, expose]
+def IterM.filterWithPostcondition {α β : Type w} {m : Type w → Type w'} {n : Type w → Type w''}
+    [Monad n] [MonadLiftT m n] [Iterator α m β] (f : β → PostconditionT n (ULift Bool))
+    (it : IterM (α := α) m β) :=
+  (it.filterMapWithPostcondition
+    (fun b => (f b).map (fun x => if x.down = true then some b else none)) : IterM n β)
 
 /--
 If `it` is an iterator, then `it.filterMapM f` is another iterator that applies a monadic
@@ -109,9 +387,9 @@ returned `Option` value.
 -/
 @[inline, expose]
 def IterM.filterMapM {α β γ : Type w} {m : Type w → Type w'} {n : Type w → Type w''}
-    [MonadLiftT m n] [Iterator α m β] (f : β → n (Option γ))
-    (it : IterM (α := α) m β) : IterM (α := FilterMap α m n (fun ⦃_⦄ => monadLift) f) n γ :=
-  IterM.InternalCombinators.filterMap (n := n) (fun ⦃_⦄ => monadLift) f it
+    [Iterator α m β] [Monad n] [MonadLiftT m n]
+    (f : β → n (Option γ)) (it : IterM (α := α) m β) :=
+  (it.filterMapWithPostcondition (fun b => PostconditionT.lift (f b)) : IterM n γ)
 
 /--
 If `it` is an iterator, then `it.mapM f` is another iterator that applies a monadic
@@ -150,7 +428,7 @@ For each value emitted by the base iterator `it`, this combinator calls `f`.
 @[inline, expose]
 def IterM.mapM {α β γ : Type w} {m : Type w → Type w'} {n : Type w → Type w''} [Iterator α m β]
     [Monad n] [MonadLiftT m n] (f : β → n γ) (it : IterM (α := α) m β) :=
-  (IterM.InternalCombinators.map (n := n) (fun ⦃_⦄ => monadLift) f it : IterM n γ)
+  (it.mapWithPostcondition (fun b => PostconditionT.lift (f b)) : IterM n γ)
 
 /--
 If `it` is an iterator, then `it.filterM f` is another iterator that applies a monadic
@@ -190,147 +468,8 @@ For each value emitted by the base iterator `it`, this combinator calls `f`.
 @[inline, expose]
 def IterM.filterM {α β : Type w} {m : Type w → Type w'} {n : Type w → Type w''} [Iterator α m β]
     [Monad n] [MonadLiftT m n] (f : β → n (ULift Bool)) (it : IterM (α := α) m β) :=
-  (it.filterMapM
-    (fun b => (if ·.down = true then some b else none) <$> f b) : IterM n β)
-
-instance FilterMap.instIterator {α β γ : Type w} {m : Type w → Type w'} {n : Type w → Type w''}
-    {lift : ⦃α : Type w⦄ → m α → n α} {f : β → n (Option γ)}
-    [Iterator α m β] [Monad n] :
-    Iterator (FilterMap α m n lift f) n γ where
-  step it :=
-    letI : MonadLift m n := ⟨lift (α := _)⟩
-    do
-      match ← it.internalState.inner.step with
-      | .yield it' out => do
-        match ← f out with
-        | none => return .skip (it'.filterMapM f)
-        | some out' => return .yield (it'.filterMapM f) out'
-      | .skip it' => return .skip (it'.filterMapM f)
-      | .done => return .done
-
-instance {α β γ : Type w} {m : Type w → Type w'} {n : Type w → Type w''} [Monad n] [Iterator α m β]
-    {lift : ⦃α : Type w⦄ → m α → n α} {f : β → n γ} :
-    Iterator (Map α m n lift f) n γ :=
-  inferInstanceAs <| Iterator (FilterMap α m n lift _) n γ
-
-private def FilterMap.instFinitenessRelation {α β γ : Type w} {m : Type w → Type w'}
-    {n : Type w → Type w''}
-    [Monad m] [MonadAttach m] [LawfulMonad m] [LawfulMonadAttach m]
-    [Monad n] [MonadAttach n] [LawfulMonad n] [LawfulMonadAttach n]
-    [Iterator α m β] {lift : ⦃α : Type w⦄ → m α → n α} [Internal.LawfulMonadLiftFunction lift]
-    {f : β → n (Option γ)} [Finite α m] :
-    FinitenessRelation (FilterMap α m n lift f) n where
-  rel := InvImage IterM.IsPlausibleSuccessorOf (FilterMap.inner ∘ IterM.internalState)
-  wf := InvImage.wf _ Finite.wf
-  subrelation {it it'} h := by
-    obtain ⟨step, hs, h⟩ := h
-    obtain ⟨step', hs', h⟩ := LawfulMonadAttach.canReturn_bind_imp' h
-    letI : MonadLift m n := ⟨lift (α := _)⟩
-    haveI : LawfulMonadLift m n :=
-      ⟨Internal.LawfulMonadLiftFunction.lift_pure, Internal.LawfulMonadLiftFunction.lift_bind⟩
-    replace hs' := LawfulMonadAttach.canReturn_liftM_imp' hs'
-    cases step', hs' using PlausibleIterStep.casesOn'
-    · obtain ⟨fx, hfx, h⟩ := LawfulMonadAttach.canReturn_bind_imp' h
-      split at h
-      · cases LawfulMonadAttach.eq_of_canReturn_pure h
-        cases hs
-        exact IterM.isPlausibleSuccessorOf_of_yield ‹_›
-      · cases LawfulMonadAttach.eq_of_canReturn_pure h
-        cases hs
-        exact IterM.isPlausibleSuccessorOf_of_yield ‹_›
-    · cases LawfulMonadAttach.eq_of_canReturn_pure h
-      cases hs
-      exact IterM.isPlausibleSuccessorOf_of_skip ‹_›
-    · cases LawfulMonadAttach.eq_of_canReturn_pure h
-      nomatch hs
-
-@[no_expose]
-instance FilterMap.instFinite {α β γ : Type w} {m : Type w → Type w'}
-    {n : Type w → Type w''}
-    [Monad m] [MonadAttach m] [LawfulMonad m] [LawfulMonadAttach m]
-    [Monad n] [MonadAttach n] [LawfulMonad n] [LawfulMonadAttach n]
-    [Iterator α m β] {lift : ⦃α : Type w⦄ → m α → n α} [Internal.LawfulMonadLiftFunction lift]
-    {f : β → n (Option γ)} [Finite α m] : Finite (FilterMap α m n lift f) n :=
-  Finite.of_finitenessRelation FilterMap.instFinitenessRelation
-
-@[no_expose]
-instance {α β γ : Type w} {m : Type w → Type w'} {n : Type w → Type w''}
-    [Monad m] [MonadAttach m] [LawfulMonad m] [LawfulMonadAttach m]
-    [Monad n] [MonadAttach n] [LawfulMonad n] [LawfulMonadAttach n]
-    [Iterator α m β] {lift : ⦃α : Type w⦄ → m α → n α} [Internal.LawfulMonadLiftFunction lift]
-    {f : β → n γ} [Finite α m] :
-    Finite (Map α m n lift f) n :=
-  Finite.of_finitenessRelation FilterMap.instFinitenessRelation
-
-private def Map.instProductivenessRelation {α β γ : Type w} {m : Type w → Type w'}
-    {n : Type w → Type w''}
-    [Monad m] [MonadAttach m] [LawfulMonad m] [LawfulMonadAttach m]
-    [Monad n] [MonadAttach n] [LawfulMonad n] [LawfulMonadAttach n]
-    [Iterator α m β] {lift : ⦃α : Type w⦄ → m α → n α} [Internal.LawfulMonadLiftFunction lift]
-    {f : β → n γ} [Productive α m] :
-    ProductivenessRelation (Map α m n lift f) n where
-  rel := InvImage IterM.IsPlausibleSkipSuccessorOf (FilterMap.inner ∘ IterM.internalState)
-  wf := InvImage.wf _ Productive.wf
-  subrelation {it it'} h := by
-    obtain ⟨step, hs, h⟩ := LawfulMonadAttach.canReturn_bind_imp' h
-    letI : MonadLift m n := ⟨lift (α := _)⟩
-    haveI : LawfulMonadLift m n :=
-      ⟨Internal.LawfulMonadLiftFunction.lift_pure, Internal.LawfulMonadLiftFunction.lift_bind⟩
-    replace hs := LawfulMonadAttach.canReturn_liftM_imp' hs
-    cases step, hs using PlausibleIterStep.casesOn'
-    · simp only [bind_map_left, bind_pure_comp] at h
-      obtain ⟨fx, hfx, h⟩ := LawfulMonadAttach.canReturn_map_imp' h
-      nomatch h
-    · cases LawfulMonadAttach.eq_of_canReturn_pure h
-      assumption
-    · nomatch LawfulMonadAttach.eq_of_canReturn_pure h
-
-@[no_expose]
-instance Map.instProductive {α β γ : Type w} {m : Type w → Type w'}
-    {n : Type w → Type w''}
-    [Monad m] [MonadAttach m] [LawfulMonad m] [LawfulMonadAttach m]
-    [Monad n] [MonadAttach n] [LawfulMonad n] [LawfulMonadAttach n]
-    [Iterator α m β] {lift : ⦃α : Type w⦄ → m α → n α} [Internal.LawfulMonadLiftFunction lift]
-    {f : β → n γ} [Productive α m] :
-    Productive (Map α m n lift f) n :=
-  Productive.of_productivenessRelation Map.instProductivenessRelation
-
-instance {α β γ : Type w} {m : Type w → Type w'}
-    {n : Type w → Type w''} {o : Type w → Type x} [Monad n] [MonadAttach n] [Monad o] [Iterator α m β]
-    {lift : ⦃α : Type w⦄ → m α → n α}
-    {f : β → n (Option γ)} :
-    IteratorCollect (FilterMap α m n lift f) n o :=
-  .defaultImplementation
-
-instance FilterMap.instIteratorLoop {α β γ : Type w} {m : Type w → Type w'}
-    {n : Type w → Type w''} {o : Type x → Type x'}
-    [Monad n] [MonadAttach n] [Monad o] [MonadAttach o] [Iterator α m β]
-    {lift : ⦃α : Type w⦄ → m α → n α} {f : β → n (Option γ)} :
-    IteratorLoop (FilterMap α m n lift f) n o :=
-  .defaultImplementation
-
-/--
-`map` operations allow for a more efficient implementation of `toArray`. For example,
-`array.iter.map f |>.toArray happens in-place if possible.
--/
-instance Map.instIteratorCollect {α β γ : Type w} {m : Type w → Type w'}
-    {n : Type w → Type w''} {o : Type w → Type x} [Monad n] [Monad o] [Iterator α m β]
-    {lift₁ : ⦃α : Type w⦄ → m α → n α}
-    {f : β → n γ} [IteratorCollect α m o] :
-    IteratorCollect (Map α m n lift₁ f) n o where
-  toArrayMapped lift₂ _ g it :=
-    letI : MonadLift m n := ⟨lift₁ (α := _)⟩
-    letI : MonadLift n o := ⟨lift₂ (δ := _)⟩
-    IteratorCollect.toArrayMapped
-      (lift := fun ⦃_⦄ => monadLift)
-      (fun x => do g (← f x))
-      it.internalState.inner (m := m)
-
-instance Map.instIteratorLoop {α β γ : Type w} {m : Type w → Type w'}
-    {n : Type w → Type w''} {o : Type x → Type x'} [Monad n] [MonadAttach n] [Monad o]
-    [MonadAttach o] [Iterator α m β] {lift : ⦃α : Type w⦄ → m α → n α} {f : β → n γ} :
-    IteratorLoop (Map α m n lift f) n o :=
-  .defaultImplementation
+  (it.filterMapWithPostcondition
+    (fun b => (PostconditionT.lift (f b)).map (if ·.down = true then some b else none)) : IterM n β)
 
 /--
 If `it` is an iterator, then `it.filterMap f` is another iterator that applies a function `f` to all
@@ -366,7 +505,7 @@ returned `Option` value.
 @[inline, expose]
 def IterM.filterMap {α β γ : Type w} {m : Type w → Type w'}
     [Iterator α m β] [Monad m] (f : β → Option γ) (it : IterM (α := α) m β) :=
-  (it.filterMapM (fun b => pure (f b)) : IterM m γ)
+  (it.filterMapWithPostcondition (fun b => pure (f b)) : IterM m γ)
 
 /--
 If `it` is an iterator, then `it.map f` is another iterator that applies a
@@ -395,7 +534,7 @@ For each value emitted by the base iterator `it`, this combinator calls `f`.
 @[inline, expose]
 def IterM.map {α β γ : Type w} {m : Type w → Type w'} [Iterator α m β] [Monad m] (f : β → γ)
     (it : IterM (α := α) m β) :=
-  (it.mapM (fun b => pure (f b)) : IterM m γ)
+  (it.mapWithPostcondition (fun b => pure (f b)) : IterM m γ)
 
 /--
 If `it` is an iterator, then `it.filter f` is another iterator that applies a
