src/Init/Data/String/Pattern/Char.lean
@@ -32,17 +32,31 @@ def iter (c : Char) (s : Slice) : Std.Iter (α := ForwardCharSearcher c s) (Sear
   { internalState := { currPos := s.startPos }}
 
 instance (s : Slice) : Std.Iterators.Iterator (ForwardCharSearcher c s) Id (SearchStep s) where
-  step
-    | ⟨⟨currPos⟩⟩ => do
-      if h1 : currPos = s.endPos then
-        return .done
+  IsPlausibleStep it
+    | .yield it' out =>
+      ∃ h1 : it.internalState.currPos ≠ s.endPos,
+        it'.internalState.currPos = it.internalState.currPos.next h1 ∧
+        match out with
+        | .matched startPos endPos =>
+          it.internalState.currPos = startPos ∧
+          it'.internalState.currPos = endPos ∧
+          it.internalState.currPos.get h1 = c
+        | .rejected startPos endPos =>
+          it.internalState.currPos = startPos ∧
+          it'.internalState.currPos = endPos ∧
+          it.internalState.currPos.get h1 ≠ c
+    | .skip _ => False
+    | .done => it.internalState.currPos = s.endPos
+  step := fun ⟨⟨currPos⟩⟩ =>
+    if h1 : currPos = s.endPos then
+      pure (.deflate ⟨.done, by simp [h1]⟩)
+    else
+      let nextPos := currPos.next h1
+      let nextIt := ⟨⟨nextPos⟩⟩
+      if h2 : currPos.get h1 = c then
+        pure (.deflate ⟨.yield nextIt (.matched currPos nextPos), by simp [h1, h2, nextIt, nextPos]⟩)
       else
-        let nextPos := currPos.next h1
-        let nextIt := ⟨⟨nextPos⟩⟩
-        if currPos.get h1 = c then
-          return .yield nextIt (.matched currPos nextPos)
-        else
-          return .yield nextIt (.rejected currPos nextPos)
+        pure (.deflate ⟨.yield nextIt (.rejected currPos nextPos), by simp [h1, h2, nextIt, nextPos]⟩)
 
 def finitenessRelation : Std.Iterators.FinitenessRelation (ForwardCharSearcher s c) Id where
   rel := InvImage WellFoundedRelation.rel (fun it => it.internalState.currPos)
@@ -50,12 +64,12 @@ def finitenessRelation : Std.Iterators.FinitenessRelation (ForwardCharSearcher s
   subrelation {it it'} h := by
     simp_wf
     obtain ⟨step, h, h'⟩ := h
-    simp only [Std.Iterators.IterM.IsPlausibleStep, MonadAttach.CanReturn,
-      Std.Iterators.Iterator.step] at h'
-    split at h'
+    cases step
+    · cases h
+      obtain ⟨_, h2, _⟩ := h'
+      simp [h2]
     · cases h'
-      cases h
-    · split at h' <;> (cases h'; cases h; simp)
+    · cases h
 
 instance : Std.Iterators.Finite (ForwardCharSearcher s c) Id :=
   .of_finitenessRelation finitenessRelation
@@ -82,17 +96,32 @@ def iter (c : Char) (s : Slice) : Std.Iter (α := BackwardCharSearcher s) (Searc
   { internalState := { currPos := s.endPos, needle := c }}
 
 instance (s : Slice) : Std.Iterators.Iterator (BackwardCharSearcher s) Id (SearchStep s) where
-  step
-    | ⟨currPos, needle⟩ => do
-      if h1 : currPos = s.startPos then
-        return .done
+  IsPlausibleStep it
+    | .yield it' out =>
+      it.internalState.needle = it'.internalState.needle ∧
+      ∃ h1 : it.internalState.currPos ≠ s.startPos,
+        it'.internalState.currPos = it.internalState.currPos.prev h1 ∧
+        match out with
+        | .matched startPos endPos =>
+          it.internalState.currPos = endPos ∧
+          it'.internalState.currPos = startPos ∧
+          (it.internalState.currPos.prev h1).get Pos.prev_ne_endPos = it.internalState.needle
+        | .rejected startPos endPos =>
+          it.internalState.currPos = endPos ∧
+          it'.internalState.currPos = startPos ∧
+          (it.internalState.currPos.prev h1).get Pos.prev_ne_endPos ≠ it.internalState.needle
+    | .skip _ => False
+    | .done => it.internalState.currPos = s.startPos
+  step := fun ⟨currPos, needle⟩ =>
+    if h1 : currPos = s.startPos then
+      pure (.deflate ⟨.done, by simp [h1]⟩)
+    else
+      let nextPos := currPos.prev h1
+      let nextIt := ⟨nextPos, needle⟩
+      if h2 : nextPos.get Pos.prev_ne_endPos = needle then
+        pure (.deflate ⟨.yield nextIt (.matched nextPos currPos), by simp [h1, h2, nextIt, nextPos]⟩)
       else
-        let nextPos := currPos.prev h1
-        let nextIt := ⟨nextPos, needle⟩
-        if nextPos.get Pos.prev_ne_endPos = needle then
-          return .yield nextIt (.matched nextPos currPos)
-        else
-          return .yield nextIt (.rejected nextPos currPos)
+        pure (.deflate ⟨.yield nextIt (.rejected nextPos currPos), by simp [h1, h2, nextIt, nextPos]⟩)
 
 def finitenessRelation : Std.Iterators.FinitenessRelation (BackwardCharSearcher s) Id where
   rel := InvImage WellFoundedRelation.rel (fun it => it.internalState.currPos.down)
@@ -100,13 +129,12 @@ def finitenessRelation : Std.Iterators.FinitenessRelation (BackwardCharSearcher 
   subrelation {it it'} h := by
     simp_wf
     obtain ⟨step, h, h'⟩ := h
-    simp only [Std.Iterators.IterM.IsPlausibleStep, MonadAttach.CanReturn,
-      Std.Iterators.Iterator.step] at h'
-    split at h'
+    cases step
+    · cases h
+      obtain ⟨_, h1, h2, _⟩ := h'
+      simp [h2]
     · cases h'
-      cases h
-    · split at h' <;> (cases h'; cases h; simp)
-    simp_wf
+    · cases h
 
 instance : Std.Iterators.Finite (BackwardCharSearcher s) Id :=
   .of_finitenessRelation finitenessRelation
