src/Init/Data/String/Pattern/Pred.lean
@@ -33,16 +33,31 @@ def iter (p : Char → Bool) (s : Slice) : Std.Iter (α := ForwardCharPredSearch
   { internalState := { currPos := s.startPos }}
 
 instance (s : Slice) : Std.Iterators.Iterator (ForwardCharPredSearcher p s) Id (SearchStep s) where
-  step := fun ⟨⟨currPos⟩⟩ => do
+  IsPlausibleStep it
+    | .yield it' out =>
+      ∃ h1 : it.internalState.currPos ≠ s.endPos,
+        it'.internalState.currPos = it.internalState.currPos.next h1 ∧
+        match out with
+        | .matched startPos endPos =>
+          it.internalState.currPos = startPos ∧
+          it'.internalState.currPos = endPos ∧
+          p (it.internalState.currPos.get h1)
+        | .rejected startPos endPos =>
+          it.internalState.currPos = startPos ∧
+          it'.internalState.currPos = endPos ∧
+          ¬ p (it.internalState.currPos.get h1)
+    | .skip _ => False
+    | .done => it.internalState.currPos = s.endPos
+  step := fun ⟨⟨currPos⟩⟩ =>
     if h1 : currPos = s.endPos then
-      return .done
+      pure (.deflate ⟨.done, by simp [h1]⟩)
     else
       let nextPos := currPos.next h1
       let nextIt := ⟨⟨nextPos⟩⟩
-      if p <| currPos.get h1 then
-        return .yield nextIt (.matched currPos nextPos)
+      if h2 : p <| currPos.get h1 then
+        pure (.deflate ⟨.yield nextIt (.matched currPos nextPos), by simp [h1, h2, nextPos, nextIt]⟩)
       else
-        return .yield nextIt (.rejected currPos nextPos)
+        pure (.deflate ⟨.yield nextIt (.rejected currPos nextPos), by simp [h1, h2, nextPos, nextIt]⟩)
 
 
 def finitenessRelation : Std.Iterators.FinitenessRelation (ForwardCharPredSearcher p s) Id where
@@ -51,13 +66,12 @@ def finitenessRelation : Std.Iterators.FinitenessRelation (ForwardCharPredSearch
   subrelation {it it'} h := by
     simp_wf
     obtain ⟨step, h, h'⟩ := h
-    simp only [Std.Iterators.IterM.IsPlausibleStep, MonadAttach.CanReturn,
-      Std.Iterators.Iterator.step] at h'
-    split at h'
+    cases step
+    · cases h
+      obtain ⟨_, h2, _⟩ := h'
+      simp [h2]
     · cases h'
-      cases h
-    · split at h' <;> (cases h'; cases h; simp)
-    simp_wf
+    · cases h
 
 instance : Std.Iterators.Finite (ForwardCharPredSearcher p s) Id :=
   .of_finitenessRelation finitenessRelation
@@ -92,16 +106,32 @@ def iter (c : Char → Bool) (s : Slice) : Std.Iter (α := BackwardCharPredSearc
   { internalState := { currPos := s.endPos, needle := c }}
 
 instance (s : Slice) : Std.Iterators.Iterator (BackwardCharPredSearcher s) Id (SearchStep s) where
-  step := fun ⟨currPos, needle⟩ => do
+  IsPlausibleStep it
+    | .yield it' out =>
+      it.internalState.needle = it'.internalState.needle ∧
+      ∃ h1 : it.internalState.currPos ≠ s.startPos,
+        it'.internalState.currPos = it.internalState.currPos.prev h1 ∧
+        match out with
+        | .matched startPos endPos =>
+          it.internalState.currPos = endPos ∧
+          it'.internalState.currPos = startPos ∧
+          it.internalState.needle ((it.internalState.currPos.prev h1).get Pos.prev_ne_endPos)
+        | .rejected startPos endPos =>
+          it.internalState.currPos = endPos ∧
+          it'.internalState.currPos = startPos ∧
+          ¬ it.internalState.needle ((it.internalState.currPos.prev h1).get Pos.prev_ne_endPos)
+    | .skip _ => False
+    | .done => it.internalState.currPos = s.startPos
+  step := fun ⟨currPos, needle⟩ =>
     if h1 : currPos = s.startPos then
-      return .done
+      pure (.deflate ⟨.done, by simp [h1]⟩)
     else
       let nextPos := currPos.prev h1
       let nextIt := ⟨nextPos, needle⟩
-      if needle <| nextPos.get Pos.prev_ne_endPos then
-        return .yield nextIt (.matched nextPos currPos)
+      if h2 : needle <| nextPos.get Pos.prev_ne_endPos then
+        pure (.deflate ⟨.yield nextIt (.matched nextPos currPos), by simp [h1, h2, nextIt, nextPos]⟩)
       else
-        return .yield nextIt (.rejected nextPos currPos)
+        pure (.deflate ⟨.yield nextIt (.rejected nextPos currPos), by simp [h1, h2, nextIt, nextPos]⟩)
 
 def finitenessRelation : Std.Iterators.FinitenessRelation (BackwardCharPredSearcher s) Id where
   rel := InvImage WellFoundedRelation.rel
@@ -110,14 +140,14 @@ def finitenessRelation : Std.Iterators.FinitenessRelation (BackwardCharPredSearc
   subrelation {it it'} h := by
     simp_wf
     obtain ⟨step, h, h'⟩ := h
-    simp only [Std.Iterators.IterM.IsPlausibleStep, MonadAttach.CanReturn,
-      Std.Iterators.Iterator.step] at h'
-    split at h'
+    cases step
+    · cases h
+      obtain ⟨_, h1, h2, _⟩ := h'
+      have h3 := Pos.offset_prev_lt_offset (h := h1)
+      simp [Pos.ext_iff, String.Pos.Raw.ext_iff, String.Pos.Raw.lt_iff] at h2 h3
+      omega
     · cases h'
-      cases h
-    · cases h'
-      have h3 := Pos.offset_prev_lt_offset (h := ‹_›)
-      split at h <;> (cases h; simpa using h3)
+    · cases h
 
 instance : Std.Iterators.Finite (BackwardCharPredSearcher s) Id :=
   .of_finitenessRelation finitenessRelation
