src/Std/Data/Iterators/Combinators/Monadic/Drop.lean
@@ -8,7 +8,6 @@ module
 prelude
 public import Init.Data.Iterators.Consumers.Loop
 public import Init.Data.Iterators.Internal.Termination
-import Init.Control.Lawful.MonadAttach.Lemmas
 
 @[expose] public section
 
@@ -58,109 +57,107 @@ does not drop any elements anymore.
 def IterM.drop (n : Nat) (it : IterM (α := α) m β) :=
   toIterM (Drop.mk n it) m β
 
-instance Drop.instIterator [Monad m] [Iterator α m β] : Iterator (Drop α m β) m β where
-  step it := do
-    match ← it.internalState.inner.step with
-    | .yield it' out =>
-      match it.internalState.remaining with
-      | 0 => return .yield (it'.drop 0) out
-      | k + 1 => return .skip (it'.drop k)
-    | .skip it' =>
-      return .skip (it'.drop it.internalState.remaining)
-    | .done =>
-      return .done
+inductive Drop.PlausibleStep [Iterator α m β] (it : IterM (α := Drop α m β) m β) :
+    (step : IterStep (IterM (α := Drop α m β) m β) β) → Prop where
+  | drop : ∀ {it' out k}, it.internalState.inner.IsPlausibleStep (.yield it' out) →
+      it.internalState.remaining = k + 1 → PlausibleStep it (.skip (it'.drop k))
+  | skip : ∀ {it'}, it.internalState.inner.IsPlausibleStep (.skip it') →
+      PlausibleStep it (.skip (it'.drop it.internalState.remaining))
+  | done : it.internalState.inner.IsPlausibleStep .done → PlausibleStep it .done
+  | yield : ∀ {it' out}, it.internalState.inner.IsPlausibleStep (.yield it' out) →
+      it.internalState.remaining = 0 → PlausibleStep it (.yield (it'.drop 0) out)
 
-private def Drop.FiniteRel (m : Type w → Type w') [MonadAttach m] [Iterator α m β] [Finite α m] :
+instance Drop.instIterator [Monad m] [Iterator α m β] : Iterator (Drop α m β) m β where
+  IsPlausibleStep := Drop.PlausibleStep
+  step it := do
+    match (← it.internalState.inner.step).inflate with
+    | .yield it' out h =>
+      match h' : it.internalState.remaining with
+      | 0 => pure <| .deflate <| .yield (it'.drop 0) out (.yield h h')
+      | k + 1 => pure <| .deflate <| .skip (it'.drop k) (.drop h h')
+    | .skip it' h =>
+      pure <| .deflate <| .skip (it'.drop it.internalState.remaining) (.skip h)
+    | .done h =>
+      pure <| .deflate <| .done (.done h)
+
+private def Drop.FiniteRel (m : Type w → Type w') [Iterator α m β] [Finite α m] :
     IterM (α := Drop α m β) m β → IterM (α := Drop α m β) m β → Prop :=
   InvImage IterM.TerminationMeasures.Finite.Rel
     (IterM.finitelyManySteps ∘ Drop.inner ∘ IterM.internalState)
 
-private def Drop.instFinitenessRelation
-    [Monad m] [MonadAttach m] [LawfulMonad m] [LawfulMonadAttach m]
-    [Iterator α m β] [Finite α m] :
+private def Drop.instFinitenessRelation [Iterator α m β] [Monad m]
+    [Finite α m] :
     FinitenessRelation (Drop α m β) m where
   rel := Drop.FiniteRel m
   wf := by
     apply InvImage.wf
     exact WellFoundedRelation.wf
   subrelation {it it'} h := by
-    obtain ⟨step, hs, h⟩ := h
-    obtain ⟨step', hs', h⟩ := LawfulMonadAttach.canReturn_bind_imp' h
-    cases step', hs' using PlausibleIterStep.casesOn'
-    · simp only at h
-      split at h
-      · cases LawfulMonadAttach.eq_of_canReturn_pure h
-        cases hs
-        exact IterM.TerminationMeasures.Finite.rel_of_yield ‹_›
-      · cases LawfulMonadAttach.eq_of_canReturn_pure h
-        cases hs
-        exact IterM.TerminationMeasures.Finite.rel_of_yield ‹_›
-    · cases LawfulMonadAttach.eq_of_canReturn_pure h
-      cases hs
-      exact IterM.TerminationMeasures.Finite.rel_of_skip ‹_›
-    · cases LawfulMonadAttach.eq_of_canReturn_pure h
-      nomatch hs
+    obtain ⟨step, h, h'⟩ := h
+    cases h'
+    case drop it' h' _ =>
+      cases h
+      apply IterM.TerminationMeasures.Finite.rel_of_yield
+      exact h'
+    case skip it' h' =>
+      cases h
+      apply IterM.TerminationMeasures.Finite.rel_of_skip
+      exact h'
+    case done h' =>
+      cases h
+    case yield it' out h' h'' =>
+      cases h
+      apply IterM.TerminationMeasures.Finite.rel_of_yield
+      exact h'
 
-instance Drop.instFinite
-    [Monad m] [MonadAttach m] [LawfulMonad m] [LawfulMonadAttach m]
-    [Iterator α m β] [Finite α m] :
+instance Drop.instFinite [Iterator α m β] [Monad m] [Finite α m] :
     Finite (Drop α m β) m :=
   by exact Finite.of_finitenessRelation instFinitenessRelation
 
-private def Drop.ProductiveRel (m : Type w → Type w')
-    [Monad m] [MonadAttach m] [Iterator α m β] [Productive α m] :
+private def Drop.ProductiveRel (m : Type w → Type w') [Iterator α m β] [Productive α m] :
     IterM (α := Drop α m β) m β → IterM (α := Drop α m β) m β → Prop :=
   InvImage (Prod.Lex Nat.lt_wfRel.rel IterM.TerminationMeasures.Productive.Rel)
     (fun it => (it.internalState.remaining, it.internalState.inner.finitelyManySkips))
 
-private theorem Drop.productiveRel_of_remaining
-    [Monad m] [MonadAttach m] [Iterator α m β] [Productive α m]
+private theorem Drop.productiveRel_of_remaining [Monad m] [Iterator α m β] [Productive α m]
     {it it' : IterM (α := Drop α m β) m β}
     (h : it'.internalState.remaining < it.internalState.remaining) : Drop.ProductiveRel m it' it :=
   Prod.Lex.left _ _ h
 
-private theorem Drop.productiveRel_of_inner
-    [Monad m] [MonadAttach m] [Iterator α m β] [Productive α m] {remaining : Nat}
+private theorem Drop.productiveRel_of_inner [Monad m] [Iterator α m β] [Productive α m] {remaining : Nat}
     {it it' : IterM (α := α) m β}
     (h : it'.finitelyManySkips.Rel it.finitelyManySkips) :
     Drop.ProductiveRel m (it'.drop remaining) (it.drop remaining) :=
   Prod.Lex.right _ h
 
-private def Drop.instProductivenessRelation
-    [Monad m] [MonadAttach m] [LawfulMonad m] [LawfulMonadAttach m]
-    [Iterator α m β] [Productive α m] :
+private def Drop.instProductivenessRelation [Iterator α m β] [Monad m]
+    [Productive α m] :
     ProductivenessRelation (Drop α m β) m where
   rel := Drop.ProductiveRel m
   wf := by
     apply InvImage.wf
     exact WellFoundedRelation.wf
   subrelation {it it'} h := by
-    obtain ⟨step, hs, h⟩ := LawfulMonadAttach.canReturn_bind_imp' h
-    cases step, hs using PlausibleIterStep.casesOn'
-    · simp only at h
-      split at h
-      · nomatch LawfulMonadAttach.eq_of_canReturn_pure h
-      · cases LawfulMonadAttach.eq_of_canReturn_pure h
-        apply productiveRel_of_remaining
-        simp [IterM.drop, *]
-    · cases LawfulMonadAttach.eq_of_canReturn_pure h
+    rw [IterM.IsPlausibleSkipSuccessorOf] at h
+    cases h
+    case drop it' out k h h' =>
+      apply productiveRel_of_remaining
+      simp [h', IterM.drop]
+    case skip it' h =>
       apply productiveRel_of_inner
       apply IterM.TerminationMeasures.Productive.rel_of_skip
-      assumption
-    · nomatch LawfulMonadAttach.eq_of_canReturn_pure h
+      exact h
 
-instance Drop.instProductive
-    [Monad m] [MonadAttach m] [LawfulMonad m] [LawfulMonadAttach m]
-    [Iterator α m β] [Productive α m] :
+instance Drop.instProductive [Iterator α m β] [Monad m] [Productive α m] :
     Productive (Drop α m β) m :=
   by exact Productive.of_productivenessRelation instProductivenessRelation
 
-instance Drop.instIteratorCollect {n : Type w → Type w'} [Monad m] [MonadAttach m] [Monad n]
-    [Iterator α m β] [Finite α m] : IteratorCollect (Drop α m β) m n :=
+instance Drop.instIteratorCollect {n : Type w → Type w'} [Monad m] [Monad n] [Iterator α m β] [Finite α m] :
+    IteratorCollect (Drop α m β) m n :=
   .defaultImplementation
 
-instance Drop.instIteratorLoop {n : Type x → Type x'} [Monad m] [MonadAttach m]
-    [Monad n] [MonadAttach n] [Iterator α m β] : IteratorLoop (Drop α m β) m n :=
+instance Drop.instIteratorLoop {n : Type x → Type x'} [Monad m] [Monad n] [Iterator α m β] :
+    IteratorLoop (Drop α m β) m n :=
   .defaultImplementation
 
 end Std.Iterators
